backends/hol4/divDefNoFixLib.sml
@@ -1,0 +1,1203 @@
+(* **DEPRECATED**: see divDefLib *)
+
+structure divDefNoFixLib :> divDefNoFixLib =
+struct
+
+open HolKernel boolLib bossLib Parse
+open boolTheory arithmeticTheory integerTheory intLib listTheory stringTheory
+
+open primitivesArithTheory primitivesBaseTacLib ilistTheory primitivesTheory
+open primitivesLib
+
+val case_result_same_eq = prove (
+  “!(r : 'a result).
+    (case r of
+       Return x => Return x
+     | Fail e => Fail e
+     | Diverge => Diverge) = r”,
+  rw [] >> CASE_TAC)
+
+(*
+val ty = id_ty
+strip_arrows ty
+*)
+
+(* TODO: move *)
+fun list_mk_arrow (tys : hol_type list) (ret_ty : hol_type) : hol_type =
+  foldr (fn (ty, aty) => ty --> aty) ret_ty tys
+
+(* TODO: move *)
+fun strip_arrows (ty : hol_type) : hol_type list * hol_type =
+  let
+    val (ty0, ty1) = dom_rng ty
+    val (tys, ret) = strip_arrows ty1
+  in
+    (ty0::tys, ret)
+  end
+  handle HOL_ERR _ => ([], ty)
+
+(* Small utilities *)
+val current_goal : term option ref = ref NONE
+
+(* Save a goal in {!current_goal} then prove it.
+
+   This way if the proof fails we can easily retrieve the goal for debugging
+   purposes.
+ *)
+fun save_goal_and_prove (g, tac) : thm =
+  let
+    val _ = current_goal := SOME g
+  in
+    prove (g, tac)
+  end
+  
+
+(*val def_qt = ‘
+(nth_fuel (n : num) (ls : 't list_t) (i : u32) : 't result =
+  case n of
+  | 0 => Loop
+  | SUC n => 
+    do case ls of
+    | ListCons x tl =>
+      if u32_to_int i = (0:int)
+      then Return x
+      else
+        do
+        i0 <- u32_sub i (int_to_u32 1);
+        nth_fuel n tl i0
+        od
+    | ListNil => 
+      Fail Failure
+    od)
+’*)
+
+val num_zero_tm = “0:num”
+val num_suc_tm = “SUC: num -> num”
+val num_ty = “:num”
+
+val fuel_def_suffix = "___fuel" (* TODO: name collisions *)
+val fuel_var_name = "$n" (* TODO: name collisions *)
+val fuel_var = mk_var (fuel_var_name, num_ty)
+val fuel_var0 = fuel_var
+val fuel_var1 = mk_var ("$m", “:num”) (* TODO: name collisions *)
+val fuel_vars_le = “^fuel_var0 <= ^fuel_var1”
+
+val fuel_predicate_suffix = "___P" (* TODO: name collisions *)
+val expand_suffix = "___E" (* TODO: name collisions *)
+
+val bool_ty = “:bool”
+
+val alpha_tyvar : hol_type = “:'a”
+val beta_tyvar : hol_type = “:'b”
+
+val is_diverge_tm = “is_diverge: 'a result -> bool”
+val diverge_tm = “Diverge : 'a result”
+
+val least_tm = “$LEAST”
+val le_tm = (fst o strip_comb) “x:num <= y:num”
+val true_tm = “T”
+val false_tm = “F”
+
+val measure_tm = “measure: ('a -> num) -> 'a -> 'a -> bool”
+
+fun mk_diverge_tm (ty : hol_type) : term =
+  let
+    val diverge_ty = mk_thy_type {Thy="primitives", Tyop="result", Args = [ty] }
+    val diverge_tm = mk_thy_const { Thy="primitives", Name="Diverge", Ty=diverge_ty }
+  in
+    diverge_tm
+  end
+
+(* Small utility: we sometimes need to generate a termination measure for
+   the fuel definitions.
+
+   We derive a measure for a type which is simply the sum of the tuples
+   of the input types of the functions.
+
+   For instance, for even and odd we have:
+   {[
+     even___fuel : num -> int -> bool result
+     odd___fuel  : num -> int -> bool result
+   ]}
+
+   So the type would be:
+   {[
+     (num # int) + (num # int)
+   ]}
+
+   Note that generally speaking we expect a type of the shape (the “:num”
+   on the left is for the fuel):
+   {[
+     (num # ...) + (num # ...) + ... + (num # ...)
+   ]}
+
+   The decreasing measure is simply given by a function which matches over
+   its argument to return the fuel, whatever the case.
+ *)
+fun mk_termination_measure_from_ty (ty : hol_type) : term =
+  let
+    val dtys = map pairSyntax.strip_prod (sumSyntax.strip_sum ty)
+    (* For every tuple, create a match to extract the num *)
+    fun mk_case_of_tuple (tys : hol_type list) : (term * term) =
+      case tys of
+        [] => failwith "mk_termination_measure_from_ty: empty list of types"
+      | [num_ty] =>
+        (* No need for a case *)
+        let val var = genvar num_ty in (var, var) end
+      | num_ty :: rem_tys =>
+        let
+          val scrut_var = genvar (pairSyntax.list_mk_prod tys)
+          val var = genvar num_ty
+          val rem_var = genvar (pairSyntax.list_mk_prod rem_tys)
+          val pats = [(pairSyntax.mk_pair (var, rem_var), var)]
+          val case_tm = TypeBase.mk_case (scrut_var, pats)
+        in
+          (scrut_var, case_tm)
+        end
+     val tuple_cases = map mk_case_of_tuple dtys
+
+    (* For every sum, create a match to extract one of the tuples *)
+    fun mk_sum_case ((tuple_var, tuple_case), (nvar, case_end)) =
+      let
+        val left_pat = sumSyntax.mk_inl (tuple_var, type_of nvar)
+        val right_pat = sumSyntax.mk_inr (nvar, type_of tuple_var)
+        val scrut = genvar (sumSyntax.mk_sum (type_of tuple_var, type_of nvar))
+        val pats = [(left_pat, tuple_case), (right_pat, case_end)]
+        val case_tm = TypeBase.mk_case (scrut, pats)
+      in
+        (scrut, case_tm)
+      end
+    val tuple_cases = rev tuple_cases
+    val (nvar, case_end) = hd tuple_cases
+    val tuple_cases = tl tuple_cases
+    val (scrut, case_tm) = foldl mk_sum_case (nvar, case_end) tuple_cases
+
+    (* Create the function *)
+    val abs_tm = mk_abs (scrut, case_tm)
+    
+    (* Add the “measure term” *)
+    val tm = inst [alpha_tyvar |-> type_of scrut] measure_tm
+    val tm = mk_comb (tm, abs_tm)
+  in
+    tm
+  end
+
+(*
+val ty = “: (num # 'a) + (num # 'b) + (num # 'c)”
+
+val tys = hd dtys
+val num_ty::rem_tys = tys
+
+val (tuple_var, tuple_case) = hd tuple_cases
+*)
+
+(* Get the smallest id which make the names unique (or to be more precise:
+   such that the names don't correspond to already defined constants).
+
+   We do this for {!mk_fuel_defs}: for some reason, the termination proof
+   fails if we try to reuse the same names as before.
+ *)
+fun get_smallest_unique_id_for_names (names : string list) : string =
+  let
+    (* Not trying to be smart here *)
+    val i : int option ref = ref NONE
+    fun get_i () = case !i of NONE => "" | SOME i => int_to_string i
+    fun incr_i () =
+      i := (case !i of NONE => SOME 0 | SOME i => SOME (i+1))
+    val continue = ref true
+    fun name_is_ok (name : string) : bool =
+      not (is_const (Parse.parse_in_context [] [QUOTE (name ^ get_i ())]))
+      handle HOL_ERR _ => false
+    val _ =
+      while !continue do (
+        let val _ = (continue := not (forall name_is_ok names)) in
+        if !continue then incr_i () else () end
+      )
+  in
+    get_i ()
+  end
+
+fun mk_fuel_defs (def_tms : term list) : thm list =
+  let
+    (* Retrieve the identifiers.
+
+       Ex.: def_tm = “even (n : int) : bool result = if i = 0 then Return T else odd (i - 1))”
+       We want to retrive: id = “even”
+     *)
+    val ids = map (fst o strip_comb o lhs) def_tms
+
+    (* In the definitions, replace the identifiers by new identifiers which use
+       fuel.
+
+       Ex.:
+       def_fuel_tm = “
+         even___fuel (fuel : nat) (n : int) : result bool =
+           case fuel of 0 => Diverge
+           | SUC fuel' => 
+             if i = 0 then Return T else odd_fuel fuel' (i - 1))”
+     *)
+     val names = map ((fn s => s ^ fuel_def_suffix) o fst o dest_var) ids
+     val index = get_smallest_unique_id_for_names names
+     fun mk_fuel_id (id : term) : term =
+       let
+         val (id_str, ty) = dest_var id
+         (* Note: we use symbols forbidden in the generation of code to
+            prevent name collisions *)
+         val fuel_id_str = id_str ^ fuel_def_suffix ^ index
+         val fuel_id = mk_var (fuel_id_str, num_ty --> ty)
+       in fuel_id end
+     val fuel_ids = map mk_fuel_id ids
+
+     val fuel_ids_with_fuel0 = map (fn id => mk_comb (id, fuel_var0)) fuel_ids
+     val fuel_ids_with_fuel1 = map (fn id => mk_comb (id, fuel_var1)) fuel_ids
+
+     (* Recurse through the terms and replace the calls *)
+     val rwr_thms0 = map (ASSUME o mk_eq) (zip ids fuel_ids_with_fuel0)
+     val rwr_thms1 = map (ASSUME o mk_eq) (zip ids fuel_ids_with_fuel1)
+
+     fun mk_fuel_tm (def_tm : term) : term =
+       let
+         val (tm0, tm1) = dest_eq def_tm
+         val tm0 = (rhs o concl o (PURE_REWRITE_CONV rwr_thms0)) tm0
+         val tm1 = (rhs o concl o (PURE_REWRITE_CONV rwr_thms1)) tm1
+       in mk_eq (tm0, tm1) end
+     val fuel_tms = map mk_fuel_tm def_tms
+
+     (* Add the case over the fuel *)
+     fun add_fuel_case (tm : term) : term =
+       let
+         val (f, body) = dest_eq tm
+         (* Create the “Diverge” term with the proper type *)
+         val body_ty = type_of body
+         val return_ty =
+           case (snd o dest_type) body_ty of [ty] => ty
+           | _ => failwith "unexpected"
+         val diverge_tm = mk_diverge_tm return_ty
+         (* Create the “SUC fuel” term *)
+         val suc_tm = mk_comb (num_suc_tm, fuel_var1)
+         val fuel_tm =
+           TypeBase.mk_case (fuel_var0, [(num_zero_tm, diverge_tm), (suc_tm, body)])
+       in mk_eq (f, fuel_tm) end
+     val fuel_tms = map add_fuel_case fuel_tms
+
+     (* Define the auxiliary definitions which use fuel *)
+     val fuel_defs_conj = list_mk_conj fuel_tms
+     (* The definition name *)
+     val def_name = (fst o dest_var o hd) fuel_ids
+     (* The tactic to prove the termination *)
+     val rty = ref “:bool” (* This is useful for debugging *)
+     fun prove_termination_tac (asms, g) =
+       let
+         val r_tm = (fst o dest_exists) g
+         val _ = rty := type_of r_tm
+         val ty = (hd o snd o dest_type) (!rty)
+         val m_tm = mk_termination_measure_from_ty ty
+       in
+         WF_REL_TAC ‘^m_tm’ (asms, g)
+       end
+
+     (* Define the fuel definitions *)
+     (*
+       val temp_def = Hol_defn def_name ‘^fuel_defs_conj’
+       Defn.tgoal temp_def
+     *)
+     val fuel_defs = tDefine def_name ‘^fuel_defs_conj’ prove_termination_tac
+   in
+     CONJUNCTS fuel_defs
+   end
+
+(*
+val (fuel_tms, fuel_defs) = mk_fuel_defs def_tms
+val fuel_def_tms = map (snd o strip_forall) ((strip_conj o concl) fuel_defs)
+val (def_tm, fuel_def_tm) = hd (zip def_tms fuel_def_tms)
+*)
+
+fun mk_is_diverge_tm (fuel_tm : term) : term =
+  case snd (dest_type (type_of fuel_tm)) of
+    [ret_ty] => mk_comb (inst [alpha_tyvar |-> ret_ty] is_diverge_tm, fuel_tm)
+   | _ => failwith "mk_is_diverge_tm: unexpected"
+
+fun mk_fuel_predicate_defs (def_tm, fuel_def_tm) : thm =
+  let
+    (* From [even i] create the term [even_P i n], where [n] is the fuel *)
+    val (id, args) = (strip_comb o lhs) def_tm
+    val (id_str, id_ty) = dest_var id
+    val (tys, ret_ty) = strip_arrows id_ty
+    val tys = append tys [num_ty]
+    val pred_ty = list_mk_arrow tys bool_ty
+    val pred_id = mk_var (id_str ^ fuel_predicate_suffix, pred_ty)
+    val pred_tm = list_mk_comb (pred_id, append args [fuel_var])
+
+    (* Create the term ~is_diverge (even_fuel n i) *)
+    val fuel_tm = lhs fuel_def_tm
+    val not_is_diverge_tm = mk_neg (mk_is_diverge_tm fuel_tm)
+
+    (* Create the term: even_P i n = ~(is_diverge (even_fuel n i) *)
+    val pred_def_tm = mk_eq (pred_tm, not_is_diverge_tm)
+  in
+    (* Create the definition *)
+    Define ‘^pred_def_tm’
+  end
+
+(*
+val (def_tm, fuel_def_tm) = hd (zip def_tms fuel_def_tms)
+
+val pred_defs = map mk_fuel_predicate_defs (zip def_tms fuel_def_tms)
+*)
+
+(* Tactic which makes progress in a proof by making a case disjunction (we use
+   this to explore all the paths in a function body). *)
+fun case_progress (asms, g) =
+  let
+    val scrut = (strip_all_cases_get_scrutinee o lhs) g
+  in Cases_on ‘^scrut’ (asms, g) end  
+
+(* Prove the fuel monotonicity properties.
+
+   We want to prove a theorem of the shape:
+   {[
+     !n m.
+       (!i. n <= m ==> even___P i n ==> even___fuel n i = even___fuel m i) /\
+       (!i. n <= m ==> odd___P i n ==> odd___fuel n i = odd___fuel m i)
+   ]}
+*)
+fun prove_fuel_mono (pred_defs : thm list) (fuel_defs : thm list) : thm =
+  let
+    val pred_tms = map (lhs o snd o strip_forall o concl) pred_defs
+    val fuel_tms = map (lhs o snd o strip_forall o concl) fuel_defs
+    val pred_fuel_tms = zip pred_tms fuel_tms
+    (* Create a set containing the names of all the functions in the recursive group *)
+    val rec_fun_set =
+      Redblackset.fromList const_name_compare (map get_fun_name_from_app fuel_tms)
+    (* Small tactic which rewrites the occurrences of recursive calls *)
+    fun rewrite_rec_call (asms, g) =
+      let
+        val scrut = (strip_all_cases_get_scrutinee o lhs) g
+        val fun_id = get_fun_name_from_app scrut (* This can fail *)
+      in
+        (* Check if the function is part of the group we are considering *)
+        if Redblackset.member (rec_fun_set, fun_id) then
+          let
+             (* Yes: use the induction hypothesis *)
+             fun apply_ind_hyp (ind_th : thm) : tactic =
+               let
+                  val th = SPEC_ALL ind_th
+                  val th_pat = (lhs o snd o strip_imp o concl) th
+                  val (var_s, ty_s) = match_term th_pat scrut
+                  (* Note that in practice the type instantiation should be empty *)
+                  val th = INST var_s (INST_TYPE ty_s th)
+               in
+                 assume_tac th
+               end
+          in
+            (last_assum apply_ind_hyp >> fs []) (asms, g)
+          end
+        else all_tac (asms, g)
+      end
+      handle HOL_ERR _ => all_tac (asms, g)
+    (* Generate terms of the shape:
+       !i. n <= m ==> even___P i n ==> even___fuel n i = even___fuel m i
+     *)
+    fun mk_fuel_eq_tm (pred_tm, fuel_tm) : term =
+      let
+        (* Retrieve the variables which are not the fuel - for the quantifiers *)
+        val vars = (tl o snd o strip_comb) fuel_tm
+        (* Introduce the fuel term which uses “m” *)
+        val m_fuel_tm = subst [fuel_var0 |-> fuel_var1] fuel_tm
+        (* Introduce the equality *)
+        val fuel_eq_tm = mk_eq (fuel_tm, m_fuel_tm)
+        (* Introduce the implication with the _P pred *)
+        val fuel_eq_tm = mk_imp (pred_tm, fuel_eq_tm)
+        (* Introduce the “n <= m ==> ...” implication *)
+        val fuel_eq_tm = mk_imp (fuel_vars_le, fuel_eq_tm)
+        (* Quantify *)
+        val fuel_eq_tm = list_mk_forall (vars, fuel_eq_tm)
+      in
+        fuel_eq_tm
+      end
+     val fuel_eq_tms = map mk_fuel_eq_tm pred_fuel_tms
+     (* Create the conjunction *)
+     val fuel_eq_tms = list_mk_conj fuel_eq_tms
+     (* Qantify over the fuels *)
+     val fuel_eq_tms = list_mk_forall ([fuel_var0, fuel_var1], fuel_eq_tms)
+     (* The tactics for the proof *)
+     val prove_tac =
+       Induct_on ‘^fuel_var0’ >-(
+         (* The ___P predicates are false: n is 0 *)
+         fs pred_defs >>
+         fs [is_diverge_def] >>
+         pure_once_rewrite_tac fuel_defs >> fs []) >>
+       (* Introduce n *)
+       gen_tac >>
+       (* Introduce m *)
+       Cases_on ‘^fuel_var1’ >-(
+         (* Contradiction: SUC n < 0 *)
+         rw [] >> exfalso >> int_tac) >>
+       fs pred_defs >>
+       fs [is_diverge_def] >>
+       pure_once_rewrite_tac fuel_defs >> fs [bind_def] >>
+       (* Introduce in the context *)
+       rpt gen_tac >>
+       (* Split the goals - note that we prove one big goal for all the functions at once *)
+       rpt strip_tac >>
+       (* Instantiate the assumption: !m. n <= m ==> ~(...)
+          with the proper m.
+        *)
+       last_x_assum imp_res_tac >>
+       (* Make sure the induction hypothesis is always the last assumption *)
+       last_x_assum assume_tac >>
+       (* Split the goals *)
+       rpt strip_tac >> fs [case_result_same_eq] >>
+       (* Explore all the paths *)
+       rpt (rewrite_rec_call >> case_progress >> fs [case_result_same_eq])
+   in
+     (* Prove *)
+     save_goal_and_prove (fuel_eq_tms, prove_tac)
+   end
+
+(*
+val fuel_mono_thm = prove_fuel_mono pred_defs fuel_defs
+
+set_goal ([], fuel_eq_tms)
+*)
+
+(* Prove the property about the least upper bound.
+
+   We want to prove theorems of the shape:
+   {[
+     (!n i. $LEAST (even___P i) <= n ==> even___fuel n i = even___fuel ($LEAST (even___P i)) i)
+   ]}
+   {[
+     (!n i. $LEAST (odd___P i) <= n ==> odd___fuel n i = odd___fuel ($LEAST (odd___P i)) i)
+   ]}
+
+   TODO: merge with other functions? (prove_pred_imp_fuel_eq_raw_thms)
+*)
+fun prove_least_fuel_mono (pred_defs : thm list) (fuel_mono_thm : thm) : thm list =
+  let
+    val thl = (CONJUNCTS o SPECL [fuel_var0, fuel_var1]) fuel_mono_thm
+    fun mk_least_fuel_thm (pred_def, mono_thm) : thm =
+      let
+        (* Retrieve the predicate, without the fuel *)
+        val pred_tm = (lhs o snd o strip_forall o concl) pred_def
+        val (pred_tm, args) = strip_comb pred_tm
+        val args = rev (tl (rev args))
+        val pred_tm = list_mk_comb (pred_tm, args)
+        (* Add $LEAST *)
+        val least_pred_tm = mk_comb (least_tm, pred_tm)
+        (* Specialize all *)
+        val vars = (fst o strip_forall o concl) mono_thm
+        val th = SPECL vars mono_thm
+        (* Substitute in the mono theorem *)
+        val th = INST [fuel_var0 |-> least_pred_tm] th
+        (* Symmetrize the equality *)
+        val th = PURE_ONCE_REWRITE_RULE [EQ_SYM_EQ] th
+        (* Quantify *)
+        val th = GENL (fuel_var1 :: vars) th
+      in
+        th
+      end
+  in
+    map mk_least_fuel_thm (zip pred_defs thl)
+  end
+
+(*
+val (pred_def, mono_thm) = hd (zip pred_defs thl)
+*)
+
+(* Prove theorems of the shape:
+
+   {[
+     !n i. even___P i n ==> $LEAST (even___P i) <= n
+   ]}
+
+   TODO: merge with other functions? (prove_pred_imp_fuel_eq_raw_thms)
+ *)
+fun prove_least_pred_thms (pred_defs : thm list) : thm list =
+  let
+    fun prove_least_pred_thm (pred_def : thm) : thm =
+      let
+        val pred_tm = (lhs o snd o strip_forall o concl) pred_def
+        val (pred_no_fuel_tm, args) = strip_comb pred_tm
+        val args = rev (tl (rev args))
+        val pred_no_fuel_tm = list_mk_comb (pred_no_fuel_tm, args)
+        (* Make the “$LEAST (even___P i)” term *)
+        val least_pred_tm = mk_comb (least_tm, pred_no_fuel_tm)
+        (* Make the inequality *)
+        val tm = list_mk_comb (le_tm, [least_pred_tm, fuel_var0])
+        (* Add the implication *)
+        val tm = mk_imp (pred_tm, tm)
+        (* Quantify *)
+        val tm = list_mk_forall (args, tm)
+        val tm = mk_forall (fuel_var0, tm)
+        (* Prove *)
+        val prove_tac =
+          rpt gen_tac >>
+          disch_tac >>
+          (* Use the "fundamental" property about $LEAST *)
+          qspec_assume ‘^pred_no_fuel_tm’ whileTheory.LEAST_EXISTS_IMP >>
+          (* Prove the premise *)
+          pop_assum sg_premise_tac >- (exists_tac fuel_var0 >> fs []) >>
+          rw [] >>
+          (* Finish the proof by contraposition *)
+          spose_not_then assume_tac >>
+          fs [not_le_eq_gt]
+      in
+        save_goal_and_prove (tm, prove_tac)
+      end
+  in
+    map prove_least_pred_thm pred_defs
+  end
+
+
+(*
+val least_pred_thms = prove_least_pred_thms pred_defs
+
+val least_pred_thm = hd least_pred_thms
+*)
+
+(* Prove theorems of the shape:
+
+   {[
+     !n i. even___P i n ==> even___P i ($LEAST (even___P i))
+   ]}
+*)
+fun prove_pred_n_imp_pred_least_thms (pred_defs : thm list) : thm list =
+  let
+    fun prove_pred_n_imp_pred_least (pred_def : thm) : thm =
+      let
+        val pred_tm = (lhs o snd o strip_forall o concl) pred_def
+        val (pred_no_fuel_tm, args) = strip_comb pred_tm
+        val args = rev (tl (rev args))
+        val pred_no_fuel_tm = list_mk_comb (pred_no_fuel_tm, args)
+        (* Make the “$LEAST (even___P i)” term *)
+        val least_pred_tm = mk_comb (least_tm, pred_no_fuel_tm)
+        (* Make the “even___P i ($LEAST (even___P i))” *)
+        val tm = subst [fuel_var0 |-> least_pred_tm] pred_tm
+        (* Add the implication *)
+        val tm = mk_imp (pred_tm, tm)
+        (* Quantify *)
+        val tm = list_mk_forall (args, tm)
+        val tm = mk_forall (fuel_var0, tm)
+        (* The proof tactic *)
+        val prove_tac =
+          rpt gen_tac >>
+          disch_tac >>
+          (* Use the "fundamental" property about $LEAST *)
+          qspec_assume ‘^pred_no_fuel_tm’ whileTheory.LEAST_EXISTS_IMP >>
+          (* Prove the premise *)
+          pop_assum sg_premise_tac >- (exists_tac fuel_var0 >> fs []) >>
+          rw []
+      in
+        save_goal_and_prove (tm, prove_tac)
+      end
+  in
+    map prove_pred_n_imp_pred_least pred_defs
+  end
+
+(*
+val (pred_def, mono_thm) = hd (zip pred_defs thl)
+val least_fuel_mono_thms = prove_least_fuel_mono pred_defs fuel_defs fuel_mono_thm
+
+val least_fuel_mono_thm = hd least_fuel_mono_thms
+*)
+
+(* Define the "raw" definitions:
+
+   {[
+     even i = if (?n. even___P i n) then even___P ($LEAST (even___P i)) i else Diverge
+   ]}
+ *)
+fun define_raw_defs (def_tms : term list) (pred_defs : thm list) (fuel_defs : thm list) : thm list =
+  let
+    fun define_raw_def (def_tm, (pred_def, fuel_def)) : thm =
+      let
+        val app = lhs def_tm
+        val pred_tm = (lhs o snd o strip_forall o concl) pred_def
+        (* Make the “?n. even___P i n” term *)
+        val exists_fuel_tm = mk_exists (fuel_var0, pred_tm)
+        (* Make the “even___fuel ($LEAST (even___P i)) i” term *)
+        val fuel_tm = (lhs o snd o strip_forall o concl) fuel_def
+        val (pred_tm, args) = strip_comb pred_tm
+        val args = rev (tl (rev args))
+        val pred_tm = list_mk_comb (pred_tm, args)
+        val least_pred_tm = mk_comb (least_tm, pred_tm)
+        val fuel_tm = subst [fuel_var0 |-> least_pred_tm] fuel_tm
+        (* Create the Diverge term *)
+        val ret_ty = (hd o snd o dest_type) (type_of app)
+        (* Create the “if then else” *)
+        val body = TypeBase.mk_case (exists_fuel_tm, [(true_tm, fuel_tm), (false_tm, mk_diverge_tm ret_ty)])
+        (* *)
+        val raw_def_tm = mk_eq (app, body)
+      in
+        Define ‘^raw_def_tm’
+      end
+  in
+    map define_raw_def (zip def_tms (zip pred_defs fuel_defs))
+  end
+
+(*
+val raw_defs = define_raw_defs def_tms pred_defs fuel_defs
+ *)
+
+(* Prove theorems of the shape:
+
+   !n i. even___P i n ==> even___fuel n i = even i
+ *)
+fun prove_pred_imp_fuel_eq_raw_defs
+  (pred_defs : thm list)
+  (fuel_def_tms : term list)
+  (least_fuel_mono_thms : thm list)
+  (least_pred_thms : thm list)
+  (pred_n_imp_pred_least_thms : thm list)
+  (raw_defs : thm list) :
+  thm list =
+  let
+    fun prove_thm (pred_def,
+                   (fuel_def_tm,
+                    (least_fuel_mono_thm,
+                     (least_pred_thm,
+                      (pred_n_imp_pred_least_thm, raw_def))))) : thm =
+      let
+        (* Generate: “even___P i n” *)
+        val pred_tm = (lhs o snd o strip_forall o concl) pred_def
+        val (pred_no_fuel_tm, args) = strip_comb pred_tm
+        val args = rev (tl (rev args))
+        (* Generate: “even___fuel n i” *)
+        val fuel_tm = lhs fuel_def_tm
+        (* Generate: “even i” *)
+        val raw_def_tm = (lhs o snd o strip_forall o concl) raw_def
+        (* Generate: “even___fuel n i = even i” *)
+        val tm = mk_eq (fuel_tm, raw_def_tm)
+        (* Add the implication *)
+        val tm = mk_imp (pred_tm, tm)
+        (* Quantify *)
+        val tm = list_mk_forall (args, tm)
+        val tm = mk_forall (fuel_var0, tm)
+        (* Prove *)
+        val prove_tac =
+          rpt gen_tac >>
+          strip_tac >>
+          fs raw_defs >>
+          (* Case on ‘?n. even___P i n’ *)
+          CASE_TAC >> fs [] >>
+          (* Use the monotonicity property *)
+          irule least_fuel_mono_thm >>
+          imp_res_tac pred_n_imp_pred_least_thm >> fs [] >>
+          irule least_pred_thm >> fs []
+      in
+        save_goal_and_prove (tm, prove_tac)
+      end
+  in
+    map prove_thm (zip pred_defs (zip fuel_def_tms (zip least_fuel_mono_thms
+                   (zip least_pred_thms (zip pred_n_imp_pred_least_thms raw_defs)))))
+  end
+
+(*
+val pred_imp_fuel_eq_raw_defs =
+  prove_pred_imp_fuel_eq_raw_defs
+    pred_defs fuel_def_tms least_fuel_mono_thms least_pred_thms
+    pred_n_imp_pred_least_thms raw_defs
+ *)
+
+
+(* Generate "expand" definitions of the following shape (we use them to
+   hide the raw function bodies, to control the rewritings):
+
+   {[
+     even___expand even odd i : bool result =
+       if i = 0 then Return T else odd (i - 1)
+   ]}
+
+   {[
+     odd___expand even odd i : bool result =
+       if i = 0 then Return F else even (i - 1)
+   ]}
+
+ *)
+fun gen_expand_defs (def_tms : term list) =
+  let
+    (* Generate the variables for “even”, “odd”, etc. *)
+    val fun_vars = map (fst o strip_comb o lhs) def_tms
+    val fun_tys = map type_of fun_vars
+    (* Generate the expansion *)
+    fun mk_def (def_tm : term) : thm =
+      let
+        val (exp_fun, args) = (strip_comb o lhs) def_tm
+        val (exp_fun_str, exp_fun_ty) = dest_var exp_fun
+        val exp_fun_str = exp_fun_str ^ expand_suffix
+        val exp_fun_ty = list_mk_arrow fun_tys exp_fun_ty
+        val exp_fun = mk_var (exp_fun_str, exp_fun_ty)
+        val exp_fun = list_mk_comb (exp_fun, fun_vars)
+        val exp_fun = list_mk_comb (exp_fun, args)
+        val tm = mk_eq (exp_fun, rhs def_tm)
+      in
+        Define ‘^tm’
+      end
+  in
+    map mk_def def_tms
+  end
+
+(*
+val def_tm = hd def_tms
+
+val expand_defs = gen_expand_defs def_tms
+*)
+
+(* Small utility:
+
+   Return the list:
+   {[
+     (“even___P i n”, “even i = even___expand even odd i”),
+     ...
+   ]}
+   
+ *)
+fun mk_termination_diverge_tms
+  (def_tms : term list)
+  (pred_defs : thm list)
+  (raw_defs : thm list)
+  (expand_defs : thm list) :
+  (term * term) list =
+  let
+    (* Create the substitution for the "expand" functions:
+       {[
+         even -> even
+         odd -> odd
+         ...
+       ]}
+
+       where on the left we have *variables* and on the right we have
+       the "raw" definitions.
+     *)
+    fun mk_fun_subst (def_tm, raw_def) =
+      let
+        val var = (fst o strip_comb o lhs) def_tm
+        val f = (fst o strip_comb o lhs o snd o strip_forall o concl) raw_def
+      in
+        (var |-> f)
+      end
+    val fun_subst = map mk_fun_subst (zip def_tms raw_defs)
+  
+    fun mk_tm (pred_def, (raw_def, expand_def)) :
+      term * term =
+      let
+        (* “even___P i n” *)
+        val pred_tm = (lhs o snd o strip_forall o concl) pred_def
+        (* “even i = even___expand even odd i” *)
+        val expand_tm = (lhs o snd o strip_forall o concl) expand_def
+        val expand_tm = subst fun_subst expand_tm
+        val fun_tm = (lhs o snd o strip_forall o concl) raw_def
+        val fun_eq_tm = mk_eq (fun_tm, expand_tm)
+      in (pred_tm, fun_eq_tm) end
+  in
+    map mk_tm (zip pred_defs (zip raw_defs expand_defs))
+  end
+
+(*
+val term_div_tms =
+  mk_termination_diverge_tms pred_defs raw_defs expand_defs
+*)
+
+(* Prove the termination lemmas:
+   
+   {[
+     !i.
+       (?n. even___P i n) ==>
+         even i = even___expand even odd i
+   ]}
+ *)
+fun prove_termination_thms
+  (term_div_tms : (term * term) list)
+  (fuel_defs : thm list)
+  (pred_defs : thm list)
+  (raw_defs : thm list)
+  (expand_defs : thm list)
+  (pred_n_imp_pred_least_thms : thm list)
+  (pred_imp_fuel_eq_raw_defs : thm list)
+  : thm list =
+  let
+    (* Create a map from functions in the recursive group to lemmas
+       to apply *)
+    fun mk_rec_fun_eq_pair (fuel_def, eq_th) =
+      let
+        val rfun = (get_fun_name_from_app o lhs o snd o strip_forall o concl) fuel_def
+      in
+        (rfun, eq_th)
+      end
+    val rec_fun_eq_map =
+      Redblackmap.fromList const_name_compare (
+        map mk_rec_fun_eq_pair
+          (zip fuel_defs pred_imp_fuel_eq_raw_defs))
+
+    (* Small tactic which rewrites the recursive calls *)
+    fun rewrite_rec_call (asms, g) =
+      let
+        val scrut = (strip_all_cases_get_scrutinee o lhs) g
+        val fun_id = get_fun_name_from_app scrut (* This can fail *)
+        (* This can raise an exception - hence the handle at the end
+           of the function *)
+        val eq_th = Redblackmap.find (rec_fun_eq_map, fun_id)
+        val eq_th = (UNDISCH_ALL o SPEC_ALL) eq_th
+        (* Match the theorem *)
+        val eq_th_tm = (lhs o concl) eq_th
+        val (var_s, ty_s) = match_term eq_th_tm scrut
+        val eq_th = INST var_s (INST_TYPE ty_s eq_th)
+        val eq_th = thm_to_conj_implies eq_th
+        (* Some tactics *)
+        val premise_tac = fs pred_defs >> fs [is_diverge_def]
+      in
+        (* Apply the theorem, prove the premise, and rewrite *)
+        (prove_premise_then premise_tac assume_tac eq_th >> fs []) (asms, g)
+      end handle NotFound => all_tac (asms, g)
+          | HOL_ERR _ => all_tac (asms, g) (* Getting the function name can also fail *)
+  
+    fun prove_one ((pred_tm, fun_eq_tm), pred_n_imp_pred_least_thm) :
+      thm =
+      let
+        (* “?n. even___P i n” *)
+        val pred_tm = mk_exists (fuel_var0, pred_tm)
+        (* “even i = even___expand even odd i” *)
+        val tm = fun_eq_tm
+        (* Add the implication *)
+        val tm = mk_imp (pred_tm, tm)
+        (* Quantify *)
+        val (_, args) = strip_comb (lhs fun_eq_tm)
+        val tm = list_mk_forall (args, tm)
+
+        (* Prove *)
+        val prove_tac =
+          rpt gen_tac >>
+          disch_tac >>
+
+          (* Expand the raw definition and get rid of the ‘?n ...’ *)
+          pure_once_rewrite_tac raw_defs >>
+          pure_asm_rewrite_tac [] >>
+
+          (* Simplify *)
+          fs [] >>
+
+          (* Prove that: “even___P i $(LEAST ...)” *)
+          imp_res_tac pred_n_imp_pred_least_thm >>
+
+          (* We don't need the ‘even___P i n’ assumption anymore: we have a more
+             precise one with the least upper bound *)
+          last_x_assum ignore_tac >>
+
+          (* Expand *)
+          fs pred_defs >>
+          fs [is_diverge_def] >>
+          fs expand_defs >>
+
+          (* We need to be a bit careful when expanding the definitions which use fuel:
+             it can make the simplifier loop. *)
+          rpt (pop_assum mp_tac) >>
+          pure_once_rewrite_tac fuel_defs >>
+          rpt disch_tac >>
+
+          (* Expand the binds *)
+          fs [bind_def, case_result_same_eq] >>
+
+          (* Explore all the paths by doing case disjunctions *)
+          rpt (rewrite_rec_call >> case_progress >> fs [case_result_same_eq])
+      in
+        save_goal_and_prove (tm, prove_tac)
+      end
+  in
+    map prove_one
+      (zip term_div_tms pred_n_imp_pred_least_thms)
+  end
+
+(*
+val termination_thms =
+  prove_termination_thms term_div_tms fuel_defs pred_defs
+    raw_defs expand_defs pred_n_imp_pred_least_thms
+    pred_imp_fuel_eq_raw_defs
+
+val ((pred_tm, fun_eq_tm), pred_n_imp_pred_least_thm) = hd (zip term_div_tms pred_n_imp_pred_least_thms)
+set_goal ([], tm)
+*)
+
+(* Prove the divergence lemmas:
+
+   {[
+     !i.
+       (!n. ~even___P i n) ==>
+        (!n. ~even___P i (SUC n)) ==>
+         even i = even___expand even odd i
+   ]}
+
+   Note that the shape of the theorem is very precise: this helps for the proof.
+   Also, by correctly ordering the assumptions, we make sure that by rewriting
+   we don't convert one of the two to “T”.
+ *)
+fun prove_divergence_thms
+  (term_div_tms : (term * term) list)
+  (fuel_defs : thm list)
+  (pred_defs : thm list)
+  (raw_defs : thm list)
+  (expand_defs : thm list)
+  : thm list =
+  let
+    (* Create a set containing the names of all the functions in the recursive group *)
+    fun get_rec_fun_id (fuel_def : thm) =
+     (get_fun_name_from_app o lhs o snd o strip_forall o concl) fuel_def
+    val rec_fun_set =
+      Redblackset.fromList const_name_compare (
+        map get_rec_fun_id raw_defs)
+
+    (* Small tactic which rewrites the recursive calls *)
+    fun rewrite_rec_call (asms, g) =
+      let
+        val scrut = (strip_all_cases_get_scrutinee o lhs) g
+        val fun_id = get_fun_name_from_app scrut (* This can fail *)
+      in
+        (* Check if the function is part of the group we are considering *)
+        if Redblackset.member (rec_fun_set, fun_id) then
+          let
+            (* Create a subgoal “odd i = Diverge” *)
+            val ret_ty = (hd o snd o dest_type o type_of) scrut
+            val g = mk_eq (scrut, mk_diverge_tm ret_ty)
+
+            (* Create a subgoal: “?n. odd___P i n”.
+
+               It is a bit cumbersome because we have to lookup the proper
+               predicate (from “odd” we need to lookup “odd___P”) and we
+               may have to perform substitutions... We hack a bit by using
+               a conversion to rewrite “odd i” to a term which contains
+               the “?n. odd___P i n” we are looking for.
+             *)
+            val exists_g = (rhs o concl) (PURE_REWRITE_CONV raw_defs scrut)
+            val (_, exists_g, _) = TypeBase.dest_case exists_g
+            (* The tactic to prove the subgoal *)
+            val prove_sg_tac =
+              pure_rewrite_tac raw_defs >>
+              Cases_on ‘^exists_g’ >> pure_asm_rewrite_tac [] >> fs [] >>
+              (* There must only remain the positive case (i.e., “?n. ...”):
+                 we have a contradiction *)
+              exfalso >>
+              (* The end of the proof is done by opening the definitions *)
+              pop_assum mp_tac >>
+              fs pred_defs >> fs [is_diverge_def]
+          in
+            (SUBGOAL_THEN g assume_tac >- prove_sg_tac >> fs []) (asms, g)
+          end
+        else all_tac (asms, g) (* Nothing to do *)
+      end handle HOL_ERR _ => all_tac (asms, g)
+  
+    fun prove_one (pred_tm, fun_eq_tm) :
+      thm =
+      let
+        (* “!n. ~even___P i n” *)
+        val neg_pred_tm = mk_neg pred_tm
+        val pred_tm = mk_forall (fuel_var0, neg_pred_tm)
+        val pred_suc_tm = subst [fuel_var0 |-> numSyntax.mk_suc fuel_var0] neg_pred_tm
+        val pred_suc_tm = mk_forall (fuel_var0, pred_suc_tm)
+
+        (* “even i = even___expand even odd i” *)
+        val tm = fun_eq_tm
+
+        (* Add the implications *)
+        val tm = list_mk_imp ([pred_tm, pred_suc_tm], tm)
+
+        (* Quantify *)
+        val (_, args) = strip_comb (lhs fun_eq_tm)
+        val tm = list_mk_forall (args, tm)
+
+        (* Prove *)
+        val prove_tac =
+          rpt gen_tac >>
+
+          pure_rewrite_tac raw_defs >>
+          rpt disch_tac >>
+
+          (* This allows to simplify the “?n. even___P i n” *)
+          fs [] >>
+          (* We don't need the last assumption anymore *)
+          last_x_assum ignore_tac >>
+
+          (* Expand *)
+          fs pred_defs >> fs [is_diverge_def] >>
+          fs expand_defs >>
+
+          (* We need to be a bit careful when expanding the definitions which use fuel:
+             it can make the simplifier loop.
+           *)
+          pop_assum mp_tac >>
+          pure_once_rewrite_tac fuel_defs  >>
+          rpt disch_tac >> fs [bind_def, case_result_same_eq] >>
+
+          (* Evaluate all the paths *)
+          rpt (rewrite_rec_call >> case_progress >> fs [case_result_same_eq])
+      in
+        save_goal_and_prove (tm, prove_tac)
+      end
+  in
+    map prove_one term_div_tms
+  end
+
+(*
+val (pred_tm, fun_eq_tm) = hd term_div_tms
+set_goal ([], tm)
+
+val divergence_thms =
+  prove_divergence_thms
+    term_div_tms
+    fuel_defs
+    pred_defs
+    raw_defs
+    expand_defs
+*)
+
+(* Prove the final lemmas:
+
+   {[
+     !i. even i = even___expand even odd i
+   ]}
+
+   Note that the shape of the theorem is very precise: this helps for the proof.
+   Also, by correctly ordering the assumptions, we make sure that by rewriting
+   we don't convert one of the two to “T”.
+ *)
+fun prove_final_eqs
+  (term_div_tms : (term * term) list)
+  (termination_thms : thm list)
+  (divergence_thms : thm list)
+  (raw_defs : thm list)
+  : thm list =
+  let
+    fun prove_one ((pred_tm, fun_eq_tm), (termination_thm, divergence_thm)) : thm =
+      let
+        val (_, args) = strip_comb (lhs fun_eq_tm)
+        val g = list_mk_forall (args, fun_eq_tm)
+        (* We make a case disjunction of the subgoal: “exists n. even___P i n” *)
+        val exists_g = (rhs o concl) (PURE_REWRITE_CONV raw_defs (lhs fun_eq_tm))
+        val (_, exists_g, _) = TypeBase.dest_case exists_g
+        val prove_tac =
+          rpt gen_tac >>
+          Cases_on ‘^exists_g’
+          >-( (* Termination *)
+             irule termination_thm >> pure_asm_rewrite_tac [])
+          (* Divergence *)
+          >> irule divergence_thm >> fs []
+          
+      in
+        save_goal_and_prove (g, prove_tac)
+      end    
+  in
+    map prove_one (zip term_div_tms (zip termination_thms divergence_thms))
+  end
+
+(*
+val termination_thm = hd termination_thms
+val divergence_thm = hd divergence_thms
+set_goal ([], g)
+*)
+
+(* The final function: define potentially diverging functions in an error monad *)
+fun DefineDiv (def_qt : term quotation) =
+  let
+    (* Parse the definitions.
+    
+       Example:
+       {[
+         (even (i : int) : bool result = if i = 0 then Return T else odd (i - 1)) /\
+         (odd (i : int) : bool result = if i = 0 then Return F else even (i - 1))
+       ]}
+     *)
+    val def_tms = (strip_conj o list_mk_conj o rev) (Defn.parse_quote def_qt)
+
+    (* Generate definitions which use some fuel
+    
+       Example:
+       {[
+         even___fuel n i =
+           case fuel of
+             0 => Diverge
+           | SUC fuel => 
+             if i = 0 then Return T else odd_fuel (i - 1))
+       ]}
+     *)
+     val fuel_defs = mk_fuel_defs def_tms
+
+     (* Generate the predicate definitions.
+     
+        {[ even___P n i = = ~is_diverge (even___fuel n i) ]}
+      *)
+     val fuel_def_tms = map (snd o strip_forall o concl) fuel_defs
+     val pred_defs = map mk_fuel_predicate_defs (zip def_tms fuel_def_tms)
+     
+     (* Prove the monotonicity property for the fuel, all at once
+
+      *)
+     val fuel_mono_thm = prove_fuel_mono pred_defs fuel_defs
+     
+     (* Prove the individual fuel functions - TODO: update
+
+        {[
+          !n i. $LEAST (even___P i) <= n ==> even___fuel n i = even___fuel ($LEAST (even___P i)) i
+        ]}
+      *)
+     val least_fuel_mono_thms = prove_least_fuel_mono pred_defs fuel_mono_thm
+
+     (*
+       {[
+         !n i. even___P i n ==> $LEAST (even___P i) <= n
+       ]}
+      *)
+     val least_pred_thms = prove_least_pred_thms pred_defs
+
+     (*
+       {[
+         !n i. even___P i n ==> even___P i ($LEAST (even___P i))
+       ]}
+      *)
+     val pred_n_imp_pred_least_thms = prove_pred_n_imp_pred_least_thms pred_defs
+
+     (*
+       "Raw" definitions:
+
+       {[
+         even i = if (?n. even___P i n) then even___P ($LEAST (even___P i)) i else Diverge
+       ]}
+      *)
+     val raw_defs = define_raw_defs def_tms pred_defs fuel_defs
+
+     (*
+       !n i. even___P i n ==> even___fuel n i = even i
+      *)
+     val pred_imp_fuel_eq_raw_defs =
+       prove_pred_imp_fuel_eq_raw_defs
+         pred_defs fuel_def_tms least_fuel_mono_thms
+         least_pred_thms pred_n_imp_pred_least_thms raw_defs
+
+     (* "Expand" definitions *)
+     val expand_defs = gen_expand_defs def_tms
+
+     (* Small utility *)
+     val term_div_tms = mk_termination_diverge_tms def_tms pred_defs raw_defs expand_defs
+
+     (* Termination theorems *)
+     val termination_thms =
+       prove_termination_thms term_div_tms fuel_defs pred_defs
+         raw_defs expand_defs pred_n_imp_pred_least_thms pred_imp_fuel_eq_raw_defs
+
+     (* Divergence theorems *)
+     val divergence_thms =
+       prove_divergence_thms term_div_tms fuel_defs pred_defs raw_defs expand_defs
+
+     (* Final theorems:
+
+        {[
+          ∀i. even i = even___E even odd i,
+          ⊢ ∀i. odd i = odd___E even odd i
+        ]}
+      *)
+     val final_eqs = prove_final_eqs term_div_tms termination_thms divergence_thms raw_defs
+     val final_eqs = map (PURE_REWRITE_RULE expand_defs) final_eqs
+  in
+    (* We return the final equations, which act as rewriting theorems *)
+    final_eqs
+  end
+
+end
