backends/hol4/divDefTheory.sig
@@ -1,0 +1,187 @@
+signature divDefTheory =
+sig
+  type thm = Thm.thm
+  
+  (*  Definitions  *)
+    val fix_def : thm
+    val fix_fuel_P_def : thm
+    val fix_fuel_def : thm
+    val is_valid_fp_body_def : thm
+  
+  (*  Theorems  *)
+    val case_result_switch_eq : thm
+    val fix_fixed_diverges : thm
+    val fix_fixed_eq : thm
+    val fix_fixed_terminates : thm
+    val fix_fuel_P_least : thm
+    val fix_fuel_compute : thm
+    val fix_fuel_eq_fix : thm
+    val fix_fuel_mono : thm
+    val fix_fuel_mono_aux : thm
+    val fix_fuel_mono_least : thm
+    val fix_fuel_not_diverge_eq_fix : thm
+    val fix_fuel_not_diverge_eq_fix_aux : thm
+    val fix_not_diverge_implies_fix_fuel : thm
+    val fix_not_diverge_implies_fix_fuel_aux : thm
+    val is_valid_fp_body_compute : thm
+  
+  val divDef_grammars : type_grammar.grammar * term_grammar.grammar
+(*
+   [primitives] Parent theory of "divDef"
+   
+   [fix_def]  Definition
+      
+      ⊢ ∀f x.
+          fix f x =
+          if ∃n. fix_fuel_P f x n then
+            fix_fuel ($LEAST (fix_fuel_P f x)) f x
+          else Diverge
+   
+   [fix_fuel_P_def]  Definition
+      
+      ⊢ ∀f x n. fix_fuel_P f x n ⇔ ¬is_diverge (fix_fuel n f x)
+   
+   [fix_fuel_def]  Definition
+      
+      ⊢ (∀f x. fix_fuel 0 f x = Diverge) ∧
+        ∀n f x. fix_fuel (SUC n) f x = f (fix_fuel n f) x
+   
+   [is_valid_fp_body_def]  Definition
+      
+      ⊢ (∀f. is_valid_fp_body 0 f ⇔ F) ∧
+        ∀n f.
+          is_valid_fp_body (SUC n) f ⇔
+          ∀x. (∀g h. f g x = f h x) ∨
+              ∃h y.
+                is_valid_fp_body n h ∧ ∀g. f g x = do z <- g y; h g z od
+   
+   [case_result_switch_eq]  Theorem
+      
+      ⊢ (case
+           case x of
+             Return y => f y
+           | Fail e => Fail e
+           | Diverge => Diverge
+         of
+           Return y => g y
+         | Fail e => Fail e
+         | Diverge => Diverge) =
+        case x of
+          Return y =>
+            (case f y of
+               Return y => g y
+             | Fail e => Fail e
+             | Diverge => Diverge)
+        | Fail e => Fail e
+        | Diverge => Diverge
+   
+   [fix_fixed_diverges]  Theorem
+      
+      ⊢ ∀N f.
+          is_valid_fp_body N f ⇒
+          ∀x. ¬(∃n. fix_fuel_P f x n) ⇒ fix f x = f (fix f) x
+   
+   [fix_fixed_eq]  Theorem
+      
+      ⊢ ∀N f. is_valid_fp_body N f ⇒ ∀x. fix f x = f (fix f) x
+   
+   [fix_fixed_terminates]  Theorem
+      
+      ⊢ ∀N f.
+          is_valid_fp_body N f ⇒
+          ∀x n. fix_fuel_P f x n ⇒ fix f x = f (fix f) x
+   
+   [fix_fuel_P_least]  Theorem
+      
+      ⊢ ∀f n x.
+          fix_fuel n f x ≠ Diverge ⇒
+          fix_fuel_P f x ($LEAST (fix_fuel_P f x))
+   
+   [fix_fuel_compute]  Theorem
+      
+      ⊢ (∀f x. fix_fuel 0 f x = Diverge) ∧
+        (∀n f x.
+           fix_fuel (NUMERAL (BIT1 n)) f x =
+           f (fix_fuel (NUMERAL (BIT1 n) − 1) f) x) ∧
+        ∀n f x.
+          fix_fuel (NUMERAL (BIT2 n)) f x =
+          f (fix_fuel (NUMERAL (BIT1 n)) f) x
+   
+   [fix_fuel_eq_fix]  Theorem
+      
+      ⊢ ∀N f.
+          is_valid_fp_body N f ⇒
+          ∀n x. fix_fuel_P f x n ⇒ fix_fuel n f x = fix f x
+   
+   [fix_fuel_mono]  Theorem
+      
+      ⊢ ∀N f.
+          is_valid_fp_body N f ⇒
+          ∀n x.
+            fix_fuel_P f x n ⇒ ∀m. n ≤ m ⇒ fix_fuel n f x = fix_fuel m f x
+   
+   [fix_fuel_mono_aux]  Theorem
+      
+      ⊢ ∀n N M g f.
+          is_valid_fp_body M f ⇒
+          is_valid_fp_body N g ⇒
+          ∀x. ¬is_diverge (g (fix_fuel n f) x) ⇒
+              ∀m. n ≤ m ⇒ g (fix_fuel n f) x = g (fix_fuel m f) x
+   
+   [fix_fuel_mono_least]  Theorem
+      
+      ⊢ ∀N f.
+          is_valid_fp_body N f ⇒
+          ∀n x.
+            fix_fuel_P f x n ⇒
+            fix_fuel n f x = fix_fuel ($LEAST (fix_fuel_P f x)) f x
+   
+   [fix_fuel_not_diverge_eq_fix]  Theorem
+      
+      ⊢ ∀N f.
+          is_valid_fp_body N f ⇒
+          ∀n x.
+            f (fix_fuel n f) x ≠ Diverge ⇒ f (fix f) x = f (fix_fuel n f) x
+   
+   [fix_fuel_not_diverge_eq_fix_aux]  Theorem
+      
+      ⊢ ∀N M g f.
+          is_valid_fp_body M f ⇒
+          is_valid_fp_body N g ⇒
+          ∀n x.
+            g (fix_fuel n f) x ≠ Diverge ⇒ g (fix f) x = g (fix_fuel n f) x
+   
+   [fix_not_diverge_implies_fix_fuel]  Theorem
+      
+      ⊢ ∀N f.
+          is_valid_fp_body N f ⇒
+          ∀x. f (fix f) x ≠ Diverge ⇒ ∃n. f (fix f) x = f (fix_fuel n f) x
+   
+   [fix_not_diverge_implies_fix_fuel_aux]  Theorem
+      
+      ⊢ ∀N M g f.
+          is_valid_fp_body M f ⇒
+          is_valid_fp_body N g ⇒
+          ∀x. g (fix f) x ≠ Diverge ⇒
+              ∃n. g (fix f) x = g (fix_fuel n f) x ∧
+                  ∀m. n ≤ m ⇒ g (fix_fuel m f) x = g (fix_fuel n f) x
+   
+   [is_valid_fp_body_compute]  Theorem
+      
+      ⊢ (∀f. is_valid_fp_body 0 f ⇔ F) ∧
+        (∀n f.
+           is_valid_fp_body (NUMERAL (BIT1 n)) f ⇔
+           ∀x. (∀g h. f g x = f h x) ∨
+               ∃h y.
+                 is_valid_fp_body (NUMERAL (BIT1 n) − 1) h ∧
+                 ∀g. f g x = do z <- g y; h g z od) ∧
+        ∀n f.
+          is_valid_fp_body (NUMERAL (BIT2 n)) f ⇔
+          ∀x. (∀g h. f g x = f h x) ∨
+              ∃h y.
+                is_valid_fp_body (NUMERAL (BIT1 n)) h ∧
+                ∀g. f g x = do z <- g y; h g z od
+   
+   
+*)
+end
