backends/hol4/divDefExampleScript.sml
@@ -1,0 +1,418 @@
+(* Manually written examples of how to use the fixed-point operator from divDefScript *)
+
+open HolKernel boolLib bossLib Parse
+open boolTheory arithmeticTheory integerTheory intLib listTheory stringTheory
+
+open primitivesArithTheory primitivesBaseTacLib ilistTheory primitivesTheory
+open primitivesLib
+open divDefTheory
+
+val _ = new_theory "divDefExample"
+
+(* Rewrite the goal once, and on the left part of the goal seen as an application *)
+fun pure_once_rewrite_left_tac ths =
+  CONV_TAC (PATH_CONV "l" (PURE_ONCE_REWRITE_CONV ths))
+
+(*=============================================
+ * Example 1: nth (simply recursive function)
+ *=============================================*)
+
+Datatype:
+  list_t =
+    ListCons 't list_t
+  | ListNil
+End
+
+(* We want to use the fixed-point operator ‘fix’ to define a function ‘nth’
+   which satisfies the following equation: *)
+
+val nth_qt = ‘
+  nth (ls : 't list_t) (i : u32) : 't result =
+    case ls of
+    | ListCons x tl =>
+      if u32_to_int i = (0:int)
+      then (Return x)
+      else
+        do
+        i0 <- u32_sub i (int_to_u32 1);
+        nth tl i0
+        od
+    | ListNil => Fail Failure
+’
+
+(* When generating a recursive definition, we apply a fixed-point operator to a
+   non-recursive function *body*, in which the recursive calls are handled to
+   a continuation. In case we define a group of mutually recursive
+   definitions, we generate *one* single body for the whole group of definitions.
+   It works as follows.
+
+   The input of the body is an enumeration: we start by branching over this input such
+   that every branch corresponds to one function in the mutually recursive group.
+   Whenever we make a recursive call, we wrap the input parameters into the proper
+   variant before calling the continuation: in effect this allows us to choose
+   the function from the group which gets evaluated.
+
+   Moreover, because of constraints on the way the fixed-point operator is defined,
+   the input of the body must have the same type as its output: we also
+   store the outputs of the functions in this big enumeration.
+
+   In order to make this work, we need to shape the body so that:
+   - input values (at call sites) and output values (when returning) are properly
+     injected into the enumeration
+   - whenever we get an output value (which is an enumeration) from a recursive
+     call, we extract the value from the proper variant of the enumeration
+
+   We encode the enumeration with a nested sum type, whose constructors
+   are ‘INL’ and ‘INR’.
+
+   In the case of ‘nth’, we generate the encoding below, with the following
+   peculiarities:
+   - the input type is ‘: ('t list_t # u32) + 't’ the same as the output type
+     (modulo the ‘:result’). ‘:'t list_t # u32’ is for the input value, while
+     ‘t’ is for the output.
+ *)
+
+val nth_body_def = Define ‘
+  nth_body
+    (* The continuation is used for the recursive calls - this is required
+       by the fixed-point operator *)
+    (f : (('t list_t # u32) + 't) -> (('t list_t # u32) + 't) result)
+    
+    (* The input. Its type is: nth input type + nth output type *)
+    (x : (('t list_t # u32) + 't)) :
+
+    (* The output type is the same as the input type - this constraint
+       comes from limitations in the way we can define the fixed-point
+       operator inside the HOL logic *)
+    (('t list_t # u32) + 't) result =
+
+    (* Destruct the input. We need this to call the proper function in case
+       of mutually recursive definitions, but also to eliminate arguments
+       which correspond to the output value (the input type is the same
+       as the output type). *)
+    case x of
+    | INL x => ( (* Input case: normal function call *)
+      (* Body of nth *)
+      let (ls, i) = x in
+      case ls of
+      | ListCons x tl =>
+        if u32_to_int i = (0:int)
+        then Return (INR x)
+        else
+          do
+          i0 <- u32_sub i (int_to_u32 1);
+          (* Recursive call: we call the continuation.
+
+             We must wrap the input (here, in INL) then extract the
+             proper output (this last part is really important in
+             case of mutually recursive definitions).
+           *)
+          x <- (case f (INL (tl, i0)) of
+                | Fail e => Fail e
+                | Diverge => Diverge
+                | Return r =>
+                  case r of
+                  | INL _ => Fail Failure
+                  | INR x => Return x);
+
+          (* Wrap the return value *)
+          Return (INR x)
+          od
+      | ListNil => Fail Failure)
+    | INR _ => (* Output case: invalid, we fail *)
+      Fail Failure
+’
+
+(* Then, we prove that the body we just defined satisfies the validity property
+   required by the fixed-point theorem.
+
+   Remark:
+   We first prove the theorem with ‘SUC (SUC n)’ where ‘n’ is a variable
+   to prevent this quantity from being rewritten to 2 during the proofs. *)
+Theorem nth_body_is_valid_aux:
+  is_valid_fp_body (SUC (SUC n)) nth_body
+Proof
+  pure_once_rewrite_tac [is_valid_fp_body_def] >>
+  gen_tac >>
+  (* Expand *)
+  fs [nth_body_def, bind_def] >>
+  (* Simply explore all paths *)
+  Cases_on ‘x’ >> fs [] >>
+  Cases_on ‘x'’ >> fs [] >>
+  Cases_on ‘q’ >> fs [] >>
+  Cases_on ‘u32_to_int r = 0’ >> fs [] >>
+  Cases_on ‘u32_sub r (int_to_u32 1)’ >> fs [] >>
+  fs [case_result_switch_eq] >>
+  (* Recursive call *)
+  disj2_tac >>
+  qexists ‘\g x. case case x of INL v => Fail Failure | INR x => Return x of
+             Return x => Return (INR x)
+           | Fail e => Fail e
+           | Diverge => Diverge’ >>
+  qexists ‘INL (l, a)’ >>
+  conj_tac
+  >-(pure_once_rewrite_tac [is_valid_fp_body_def] >> fs []) >>
+  gen_tac >>
+  (* Explore all paths *)
+  Cases_on ‘g (INL (l,a))’ >> fs [] >>
+  Cases_on ‘a'’ >> fs []
+QED
+
+Theorem nth_body_is_valid:
+  is_valid_fp_body (SUC (SUC 0)) nth_body
+Proof
+  irule nth_body_is_valid_aux
+QED
+
+(* We can now define ‘nth’ in terms of the fixed-point operator applied to ‘nth_body’.
+
+   Important points:
+   - we apply ‘fix’ to ‘fix_body’
+   - we wrap the input to take the proper branch (‘INL (ls, i)’)
+   - we extract the output to have a function with the proper output type
+
+   This definition satisfies the equation we want (see next theorem). *)
+val nth_raw_def = Define ‘
+  nth (ls : 't list_t) (i : u32) =
+    case fix nth_body (INL (ls, i)) of
+    | Fail e => Fail e
+    | Diverge => Diverge
+    | Return r =>
+      case r of
+      | INL _ => Fail Failure
+      | INR x => Return x
+’
+
+(* We finally prove the target unfolding equation for ‘nth’ *)
+Theorem nth_def:
+  ∀ls i. nth (ls : 't list_t) (i : u32) : 't result =
+    case ls of
+    | ListCons x tl =>
+      if u32_to_int i = (0:int)
+      then (Return x)
+      else
+        do
+        i0 <- u32_sub i (int_to_u32 1);
+        nth tl i0
+        od
+    | ListNil => Fail Failure
+Proof
+  rpt strip_tac >>
+  (* Expand the raw definition *)
+  pure_rewrite_tac [nth_raw_def] >>
+  (* Use the fixed-point equality - the rewrite must only be applied *on the left* of the equality, in the goal *)
+  pure_once_rewrite_left_tac [HO_MATCH_MP fix_fixed_eq nth_body_is_valid] >>
+  (* Expand the body definition *)
+  pure_rewrite_tac [nth_body_def] >>
+  (* Explore all the paths - maybe we can be smarter, but this is fast and really easy *)
+  fs [bind_def] >>
+  Cases_on ‘ls’ >> fs [] >>
+  Cases_on ‘u32_to_int i = 0’ >> fs [] >>
+  Cases_on ‘u32_sub i (int_to_u32 1)’ >> fs [] >>
+  Cases_on ‘fix nth_body (INL (l,a))’ >> fs [] >>
+  Cases_on ‘a'’ >> fs []
+QED
+
+(*=======================================================*
+ * Example 2: even, odd (mutually recursive definitions)
+ *=======================================================*)
+
+(* We consider the following group of mutually recursive definitions: *)
+
+val even_odd_qt = Defn.parse_quote ‘
+ (even (i : int) : bool result = if i = 0 then Return T else odd (i - 1)) /\
+ (odd (i : int) : bool result = if i = 0 then Return F else even (i - 1))
+’
+
+(* Similarly to ‘nth’, we need to introduce a body on which to apply the
+   fixed-point operator. Here, the body is slightly more complex because
+   we have mutually recursive functions.
+
+   In particular, the input/output types is a sum of 4 types:
+   input of even + output of even + input of odd + output of odd
+   
+   That is: ‘: int + bool + int + bool’
+
+   As a consequence, the body is a case with 4 branches.
+ *)
+
+val even_odd_body_def = Define ‘
+  even_odd_body
+    (* The body takes a continuation - required by the fixed-point operator *)
+    (f : (int + bool + int + bool) -> (int + bool + int + bool) result)
+
+    (* The type of the input is:
+       input of even + output of even + input of odd + output of odd *)
+    (x : int + bool + int + bool) :
+
+    (* The output type is the same as the input type - this constraint
+       comes from limitations in the way we can define the fixed-point
+       operator inside the HOL logic *)
+    (int + bool + int + bool) result =
+
+  (* Case disjunction over the input, in order to figure out which
+     function from the group is actually called (even, or odd). *)
+  case x of
+  | INL i => (* Input of even *)
+    (* Body of even *)
+    if i = 0 then Return (INR (INL T))
+    else
+      (* Recursive calls are calls to the continuation f, wrapped
+         in the proper variant: here we call odd *)
+      (case f (INR (INR (INL (i - 1)))) of
+       | Fail e => Fail e
+       | Diverge => Diverge
+       | Return r =>
+         (* Extract the proper value from the enumeration: here, the
+            call is tail-call so this is not really necessary, but we
+            might need to retrieve the output of the call to odd, which
+            is a boolean, and do something more complex with it. *)
+         case r of
+         | INL _ => Fail Failure
+         | INR (INL _) => Fail Failure
+         | INR (INR (INL _)) => Fail Failure
+         | INR (INR (INR b)) => (* Extract the output of odd *)
+           (* Return: inject into the variant for the output of even *)
+           Return (INR (INL b))
+         )
+  | INR (INL _) => (* Output of even *)
+    (* We must ignore this one *)
+    Fail Failure
+  | INR (INR (INL i)) =>
+    (* Body of odd *)
+    if i = 0 then Return (INR (INR (INR F)))
+    else
+      (* Call to even *)
+      (case f (INL (i - 1)) of
+       | Fail e => Fail e
+       | Diverge => Diverge
+       | Return r =>
+         (* Extract the proper value from the enumeration *)
+         case r of
+         | INL _ => Fail Failure
+         | INR (INL b) => (* Extract the output of even *)
+           (* Return: inject into the variant for the output of odd *)
+           Return (INR (INR (INR b)))
+         | INR (INR (INL _)) => Fail Failure
+         | INR (INR (INR _)) => Fail Failure
+         )
+  | INR (INR (INR _)) => (* Output of odd *)
+    (* We must ignore this one *)
+    Fail Failure
+’
+
+(* We then prove that this body satisfies the validity condition *)
+Theorem even_odd_body_is_valid_aux:
+  is_valid_fp_body (SUC (SUC n)) even_odd_body
+Proof
+  pure_once_rewrite_tac [is_valid_fp_body_def] >>
+  gen_tac >>
+  (* Expand *)
+  fs [even_odd_body_def, bind_def] >>
+  (* Explore the body *)
+  Cases_on ‘x’ >> fs []
+  >-(
+    Cases_on ‘x' = 0’ >> fs [] >>
+    (* Recursive call *)
+    disj2_tac >>
+    qexists ‘\g x. case x of
+              | INL v => Fail Failure
+              | INR (INL v2) => Fail Failure
+              | INR (INR (INL v4)) => Fail Failure
+              | INR (INR (INR b)) => Return (INR (INL b))’ >>
+    qexists ‘INR (INR (INL (x' − 1)))’ >>
+    conj_tac
+    >-(pure_once_rewrite_tac [is_valid_fp_body_def] >> fs []) >>
+    fs []) >>
+  Cases_on ‘y’ >> fs [] >>
+  Cases_on ‘y'’ >> fs [] >>
+  Cases_on ‘x = 0’ >> fs []  >>
+  (* Recursive call *)
+  disj2_tac >>
+  qexists ‘\g x. case x of
+                   INL v => Fail Failure
+                 | INR (INL b) => Return (INR (INR (INR b)))
+                 | INR (INR v3) => Fail Failure’ >>
+  qexists ‘INL (x − 1)’ >>
+  conj_tac
+  >-(pure_once_rewrite_tac [is_valid_fp_body_def] >> fs []) >>
+  fs []
+QED
+
+Theorem even_odd_body_is_valid:
+  is_valid_fp_body (SUC (SUC 0)) even_odd_body
+Proof
+  irule even_odd_body_is_valid_aux
+QED
+
+(* We finally introduce the definitions for even and odd *)
+val even_raw_def = Define ‘
+  even (i : int) =
+    case fix even_odd_body (INL i) of
+    | Fail e => Fail e
+    | Diverge => Diverge
+    | Return r =>
+      case r of
+      | INL _ => Fail Failure
+      | INR (INL b) => Return b
+      | INR (INR (INL b)) => Fail Failure
+      | INR (INR (INR _)) => Fail Failure
+’
+
+val odd_raw_def = Define ‘
+  odd (i : int) =
+    case fix even_odd_body (INR (INR (INL i))) of
+    | Fail e => Fail e
+    | Diverge => Diverge
+    | Return r =>
+      case r of
+      | INL _ => Fail Failure
+      | INR (INL _) => Fail Failure
+      | INR (INR (INL _)) => Fail Failure
+      | INR (INR (INR b)) => Return b
+’
+
+Theorem even_def:
+  ∀i. even (i : int) : bool result =
+    if i = 0 then Return T else odd (i - 1)
+Proof
+  gen_tac >>
+  (* Expand the definition *)
+  pure_once_rewrite_tac [even_raw_def] >>
+  (* Use the fixed-point equality *)
+  pure_once_rewrite_left_tac [HO_MATCH_MP fix_fixed_eq even_odd_body_is_valid] >>
+  (* Expand the body definition *)
+  pure_rewrite_tac [even_odd_body_def] >>
+  (* Expand all the definitions from the group *)
+  pure_rewrite_tac [even_raw_def, odd_raw_def] >>
+  (* Explore all the paths - maybe we can be smarter, but this is fast and really easy *)
+  fs [bind_def] >>
+  Cases_on ‘i = 0’ >> fs [] >>
+  Cases_on ‘fix even_odd_body (INR (INR (INL (i − 1))))’ >> fs [] >>
+  Cases_on ‘a’ >> fs [] >>
+  Cases_on ‘y’ >> fs [] >>
+  Cases_on ‘y'’ >> fs []
+QED
+
+Theorem odd_def:
+  ∀i. odd (i : int) : bool result =
+    if i = 0 then Return F else even (i - 1)
+Proof
+  gen_tac >>
+  (* Expand the definition *)
+  pure_once_rewrite_tac [odd_raw_def] >>
+  (* Use the fixed-point equality *)
+  pure_once_rewrite_left_tac [HO_MATCH_MP fix_fixed_eq even_odd_body_is_valid] >>
+  (* Expand the body definition *)
+  pure_rewrite_tac [even_odd_body_def] >>
+  (* Expand all the definitions from the group *)
+  pure_rewrite_tac [even_raw_def, odd_raw_def] >>
+  (* Explore all the paths - maybe we can be smarter, but this is fast and really easy *)
+  fs [bind_def] >>
+  Cases_on ‘i = 0’ >> fs [] >>
+  Cases_on ‘fix even_odd_body (INL (i − 1))’ >> fs [] >>
+  Cases_on ‘a’ >> fs [] >>
+  Cases_on ‘y’ >> fs []
+QED
+
+val _ = export_theory ()
