backends/hol4/divDefLib.sml
@@ -1,5 +1,3 @@
-(* This file implements utilities to define potentially diverging functions *)
-
 structure divDefLib :> divDefLib =
 struct
 
@@ -8,1196 +6,889 @@ open boolTheory arithmeticTheory integerTheory intLib listTheory stringTheory
 
 open primitivesArithTheory primitivesBaseTacLib ilistTheory primitivesTheory
 open primitivesLib
+open divDefTheory
 
-val case_result_same_eq = prove (
-  “!(r : 'a result).
-    (case r of
-       Return x => Return x
-     | Fail e => Fail e
-     | Diverge => Diverge) = r”,
-  rw [] >> CASE_TAC)
+val dbg = ref false
+fun print_dbg s = if (!dbg) then print s else ()
 
-(*
-val ty = id_ty
-strip_arrows ty
-*)
-
-(* TODO: move *)
-fun list_mk_arrow (tys : hol_type list) (ret_ty : hol_type) : hol_type =
-  foldr (fn (ty, aty) => ty --> aty) ret_ty tys
-
-(* TODO: move *)
-fun strip_arrows (ty : hol_type) : hol_type list * hol_type =
-  let
-    val (ty0, ty1) = dom_rng ty
-    val (tys, ret) = strip_arrows ty1
-  in
-    (ty0::tys, ret)
-  end
-  handle HOL_ERR _ => ([], ty)
-
-(* Small utilities *)
-val current_goal : term option ref = ref NONE
-
-(* Save a goal in {!current_goal} then prove it.
-
-   This way if the proof fails we can easily retrieve the goal for debugging
-   purposes.
- *)
-fun save_goal_and_prove (g, tac) : thm =
-  let
-    val _ = current_goal := SOME g
-  in
-    prove (g, tac)
-  end
-  
-
-(*val def_qt = ‘
-(nth_fuel (n : num) (ls : 't list_t) (i : u32) : 't result =
-  case n of
-  | 0 => Loop
-  | SUC n => 
-    do case ls of
-    | ListCons x tl =>
-      if u32_to_int i = (0:int)
-      then Return x
-      else
-        do
-        i0 <- u32_sub i (int_to_u32 1);
-        nth_fuel n tl i0
-        od
-    | ListNil => 
-      Fail Failure
-    od)
-’*)
-
-val num_zero_tm = “0:num”
-val num_suc_tm = “SUC: num -> num”
+val result_ty = “:'a result”
+val error_ty = “:error”
+val alpha_ty = “:'a”
 val num_ty = “:num”
 
-val fuel_def_suffix = "___fuel" (* TODO: name collisions *)
-val fuel_var_name = "$n" (* TODO: name collisions *)
-val fuel_var = mk_var (fuel_var_name, num_ty)
-val fuel_var0 = fuel_var
-val fuel_var1 = mk_var ("$m", “:num”) (* TODO: name collisions *)
-val fuel_vars_le = “^fuel_var0 <= ^fuel_var1”
+val zero_num_tm = “0:num”
+val suc_tm = “SUC”
 
-val fuel_predicate_suffix = "___P" (* TODO: name collisions *)
-val expand_suffix = "___E" (* TODO: name collisions *)
-
-val bool_ty = “:bool”
-
-val alpha_tyvar : hol_type = “:'a”
-val beta_tyvar : hol_type = “:'b”
-
-val is_diverge_tm = “is_diverge: 'a result -> bool”
+val return_tm = “Return : 'a -> 'a result”
+val fail_tm = “Fail : error -> 'a result”
+val fail_failure_tm = “Fail Failure : 'a result”
 val diverge_tm = “Diverge : 'a result”
 
-val least_tm = “$LEAST”
-val le_tm = (fst o strip_comb) “x:num <= y:num”
-val true_tm = “T”
-val false_tm = “F”
+val fix_tm = “fix”
+val is_valid_fp_body_tm = “is_valid_fp_body”
 
-val measure_tm = “measure: ('a -> num) -> 'a -> 'a -> bool”
-
-fun mk_diverge_tm (ty : hol_type) : term =
+fun mk_result (ty : hol_type) : hol_type = Type.type_subst [ alpha_ty |-> ty ] result_ty
+fun dest_result (ty : hol_type) : hol_type =
   let
-    val diverge_ty = mk_thy_type {Thy="primitives", Tyop="result", Args = [ty] }
-    val diverge_tm = mk_thy_const { Thy="primitives", Name="Diverge", Ty=diverge_ty }
+    val {Args=out_ty, Thy=thy, Tyop=tyop} = dest_thy_type ty
   in
-    diverge_tm
+    if thy = "primitives" andalso tyop = "result" then hd out_ty
+    else failwith "dest_result: not a result"
   end
 
-(* Small utility: we sometimes need to generate a termination measure for
-   the fuel definitions.
+fun mk_return (x : term) : term = mk_icomb (return_tm, x)
+fun mk_fail (ty : hol_type) (e : term) : term = mk_comb (inst [ alpha_ty |-> ty ] fail_tm, e)
+fun mk_fail_failure (ty : hol_type) : term = inst [ alpha_ty |-> ty ] fail_failure_tm
+fun mk_diverge (ty : hol_type) : term = inst [ alpha_ty |-> ty ] diverge_tm
 
-   We derive a measure for a type which is simply the sum of the tuples
-   of the input types of the functions.
+fun mk_suc (n : term) = mk_comb (suc_tm, n)
 
-   For instance, for even and odd we have:
+fun enumerate (ls : 'a list) : (int * 'a) list =
+  zip (List.tabulate (List.length ls, fn i => i)) ls
+
+(*=============================================================================*
+ *
+ * Generate the (non-recursive) body to give to the fixed-point operator
+ *
+ * ============================================================================*)
+
+(* Small helper to generate wrappers of the shape: ‘INL x’, ‘INR (INL x)’, etc.
+   Note that we should have: ‘length before_tys + 1 + length after tys >= 2’
+
+   Ex.:
+   ====
+   The enumeration has type: “: 'a + 'b + 'c + 'd”.
+   We want to generate the variant which injects “x:'c” into this enumeration.
+
+   We need to split the list of types into:
    {[
-     even___fuel : num -> int -> bool result
-     odd___fuel  : num -> int -> bool result
+     before_tys = [“:'a”, “'b”]
+     tm = “x: 'c”
+     after_tys = [“:'d”]
    ]}
 
-   So the type would be:
+   The function will generate:
    {[
-     (num # int) + (num # int)
+     INR (INR (INL x) : 'a + 'b + 'c + 'd
    ]}
 
-   Note that generally speaking we expect a type of the shape (the “:num”
-   on the left is for the fuel):
-   {[
-     (num # ...) + (num # ...) + ... + (num # ...)
-   ]}
+   (* Debug *)
+   val before_tys = [“:'a”, “:'b”, “:'c”]
+   val tm = “x:'d”
+   val after_tys = [“:'e”, “:'f”]
 
-   The decreasing measure is simply given by a function which matches over
-   its argument to return the fuel, whatever the case.
+   val before_tys = [“:'a”, “:'b”, “:'c”]
+   val tm = “x:'d”
+   val after_tys = []
+
+   mk_inl_inr_wrapper before_tys tm after_tys
  *)
-fun mk_termination_measure_from_ty (ty : hol_type) : term =
+fun list_mk_inl_inr (before_tys : hol_type list) (tm : term) (after_tys : hol_type list) :
+  term =
   let
-    val dtys = map pairSyntax.strip_prod (sumSyntax.strip_sum ty)
-    (* For every tuple, create a match to extract the num *)
-    fun mk_case_of_tuple (tys : hol_type list) : (term * term) =
-      case tys of
-        [] => failwith "mk_termination_measure_from_ty: empty list of types"
-      | [num_ty] =>
-        (* No need for a case *)
-        let val var = genvar num_ty in (var, var) end
-      | num_ty :: rem_tys =>
+    val (before_tys, pat) =
+      if after_tys = []
+      then
         let
-          val scrut_var = genvar (pairSyntax.list_mk_prod tys)
-          val var = genvar num_ty
-          val rem_var = genvar (pairSyntax.list_mk_prod rem_tys)
-          val pats = [(pairSyntax.mk_pair (var, rem_var), var)]
-          val case_tm = TypeBase.mk_case (scrut_var, pats)
+          val just_before_ty = List.last before_tys
+          val before_tys = List.take (before_tys, List.length before_tys - 1)
+          val pat = sumSyntax.mk_inr (tm, just_before_ty)
         in
-          (scrut_var, case_tm)
+          (before_tys, pat)
         end
-     val tuple_cases = map mk_case_of_tuple dtys
-
-    (* For every sum, create a match to extract one of the tuples *)
-    fun mk_sum_case ((tuple_var, tuple_case), (nvar, case_end)) =
-      let
-        val left_pat = sumSyntax.mk_inl (tuple_var, type_of nvar)
-        val right_pat = sumSyntax.mk_inr (nvar, type_of tuple_var)
-        val scrut = genvar (sumSyntax.mk_sum (type_of tuple_var, type_of nvar))
-        val pats = [(left_pat, tuple_case), (right_pat, case_end)]
-        val case_tm = TypeBase.mk_case (scrut, pats)
-      in
-        (scrut, case_tm)
-      end
-    val tuple_cases = rev tuple_cases
-    val (nvar, case_end) = hd tuple_cases
-    val tuple_cases = tl tuple_cases
-    val (scrut, case_tm) = foldl mk_sum_case (nvar, case_end) tuple_cases
-
-    (* Create the function *)
-    val abs_tm = mk_abs (scrut, case_tm)
-    
-    (* Add the “measure term” *)
-    val tm = inst [alpha_tyvar |-> type_of scrut] measure_tm
-    val tm = mk_comb (tm, abs_tm)
+      else (before_tys, sumSyntax.mk_inl (tm, sumSyntax.list_mk_sum after_tys))
+    val pat = foldr (fn (ty, pat) => sumSyntax.mk_inr (pat, ty)) pat before_tys
   in
-    tm
+    pat
   end
 
-(*
-val ty = “: (num # 'a) + (num # 'b) + (num # 'c)”
+(* This function wraps a term into the proper variant of the input/output
+   sum.
 
-val tys = hd dtys
-val num_ty::rem_tys = tys
+   Ex.:
+   ====
+   For the input of the first function, we generate: ‘INL x’
+   For the output of the first function, we generate: ‘INR (INL x)’
+   For the input of the 2nd function, we generate: ‘INR (INR (INL x))’
+   etc.
 
-val (tuple_var, tuple_case) = hd tuple_cases
-*)
+   If ‘is_input’ is true: we are wrapping an input. Otherwise we are wrapping
+   an output.
 
-(* Get the smallest id which make the names unique (or to be more precise:
-   such that the names don't correspond to already defined constants).
-
-   We do this for {!mk_fuel_defs}: for some reason, the termination proof
-   fails if we try to reuse the same names as before.
+   (* Debug *)
+   val tys = [(“:'a”, “:'b”), (“:'c”, “:'d”), (“:'e”, “:'f”)]
+   val j = 1
+   val tm = “x:'c”
+   val tm = “y:'d”
+   val is_input = true
  *)
-fun get_smallest_unique_id_for_names (names : string list) : string =
+fun inject_in_param_sum (tys : (hol_type * hol_type) list) (j : int) (is_input : bool)
+  (tm : term) : term =
   let
-    (* Not trying to be smart here *)
-    val i : int option ref = ref NONE
-    fun get_i () = case !i of NONE => "" | SOME i => int_to_string i
-    fun incr_i () =
-      i := (case !i of NONE => SOME 0 | SOME i => SOME (i+1))
-    val continue = ref true
-    fun name_is_ok (name : string) : bool =
-      not (is_const (Parse.parse_in_context [] [QUOTE (name ^ get_i ())]))
-      handle HOL_ERR _ => false
-    val _ =
-      while !continue do (
-        let val _ = (continue := not (forall name_is_ok names)) in
-        if !continue then incr_i () else () end
-      )
+    fun flatten ls = List.concat (map (fn (x, y) => [x, y]) ls)
+    val before_tys = flatten (List.take (tys, j))
+    val (input_ty, output_ty) = List.nth (tys, j)
+    val after_tys = flatten (List.drop (tys, j + 1))
+    val (before_tys, after_tys) =
+      if is_input then (before_tys, output_ty :: after_tys)
+      else (before_tys @ [input_ty], after_tys)
   in
-    get_i ()
+    list_mk_inl_inr before_tys tm after_tys
   end
 
-fun mk_fuel_defs (def_tms : term list) : thm list =
+(* Remark: the order of the branches when creating matches is important.
+   For instance, in the case of ‘result’ it must be: ‘Return’, ‘Fail’, ‘Diverge’.
+
+   For the purpose of stability and maintainability, we introduce this small helper
+   which reorders the cases in a pattern before actually creating the case
+   expression.
+ *)
+fun unordered_mk_case (scrut: term, pats: (term * term) list) : term =
   let
-    (* Retrieve the identifiers.
+    (* Retrieve the constructors *)
+    val cl = TypeBase.constructors_of (type_of scrut)
+    (* Retrieve the names of the constructors *)
+    val names = map (fst o dest_const) cl
+    (* Use those to reorder the patterns *)
+    fun is_pat (name : string) (pat, _) =
+      let
+        val app = (fst o strip_comb) pat
+        val app_name = (fst o dest_const) app
+      in
+        app_name = name
+      end
+    val pats = map (fn name => valOf (List.find (is_pat name) pats)) names
+  in
+    (* Create the case *)
+    TypeBase.mk_case (scrut, pats)
+  end
 
-       Ex.: def_tm = “even (n : int) : bool result = if i = 0 then Return T else odd (i - 1))”
-       We want to retrive: id = “even”
+(* Wrap a term of type “:'a result” into a ‘case of’ which matches over
+   the result.
+
+   Ex.:
+   ====
+   {[
+     f x
+
+       ~~>
+
+     case f x of
+     | Fail e => Fail e
+     | Diverge => Diverge
+     | Return y => ... (* The branch content is generated by the continuation *)
+   ]}
+
+   ‘gen_ret_branch’ is a *continuation* which generates the content of the
+   ‘Return’ branch (i.e., the content of the ‘...’ in the example above).
+   It receives as input the value contained by the ‘Return’ (i.e., the variable
+   ‘y’ in the example above).
+
+   Remark.: the type of the term generated by ‘gen_ret_branch’ must have
+   the type ‘result’, but it can change the content of the result (i.e.,
+   if ‘scrut’ has type ‘:'a result’, we can change the type of the wrapped
+   expression to ‘:'b result’).
+
+   (* Debug *)
+   val scrut = “x: int result”
+   fun gen_ret_branch x = mk_return x
+
+   val scrut = “x: int result”
+   fun gen_ret_branch _ = “Return T”
+
+   mk_result_case scrut gen_ret_branch
+ *)
+fun mk_result_case (scrut : term) (gen_ret_branch : term -> term) : term =
+  let
+    val scrut_ty = dest_result (type_of scrut)
+    (* Return branch *)
+    val ret_var = genvar scrut_ty
+    val ret_pat = mk_return ret_var
+    val ret_br = gen_ret_branch ret_var
+    val ret_ty = dest_result (type_of ret_br)
+    (* Failure branch *)
+    val fail_var = genvar error_ty
+    val fail_pat = mk_fail scrut_ty fail_var
+    val fail_br = mk_fail ret_ty fail_var
+    (* Diverge branch *)
+    val div_pat = mk_diverge scrut_ty
+    val div_br = mk_diverge ret_ty
+  in
+    unordered_mk_case (scrut, [(ret_pat, ret_br), (fail_pat, fail_br), (div_pat, div_br)])
+  end
+
+(* Generate a ‘case ... of’ over a sum type.
+
+   Ex.:
+   ====
+   If the scrutinee is: “x : 'a + 'b + 'c” (i.e., the tys list is: [“:'a”, “:b”, “:c”]),
+   we generate:
+
+   {[
+     case x of
+     | INL y0 => ... (* Branch of index 0 *)
+     | INR (INL y1) => ... (* Branch of index 1 *)
+     | INR (INR (INL y2)) => ... (* Branch of index 2 *)
+     | INR (INR (INR y3)) => ... (* Branch of index 3 *)
+   ]}
+
+   The content of the branches is generated by the ‘gen_branch’ continuation,
+   which receives as input the index of the branch as well as the variable
+   introduced by the pattern (in the example above: ‘y0’ for the branch 0,
+   ‘y1’ for the branch 1, etc.)
+
+   (* Debug *)
+   val tys = [“:'a”, “:'b”]
+   val scrut = mk_var ("x", sumSyntax.list_mk_sum tys)
+   fun gen_branch i (x : term) = “F”
+
+   val tys = [“:'a”, “:'b”, “:'c”, “:'d”]
+   val scrut = mk_var ("x", sumSyntax.list_mk_sum tys)
+   fun gen_branch i (x : term) = if type_of x = “:'c” then mk_return x else mk_fail_failure “:'c”
+
+   list_mk_sum_case scrut tys gen_branch
+ *)
+(* For debugging *)
+val list_mk_sum_case_case = ref (“T”, [] : (term * term) list)
+(*
+val (scrut, [(pat1, br1), (pat2, br2)]) = !list_mk_sum_case_case
+*)
+fun list_mk_sum_case (scrut : term) (tys : hol_type list)
+  (gen_branch : int -> term -> term) : term =
+  let
+    (* Create the cases. Note that without sugar, the match actually looks like this:
+       {[
+         case x of
+         | INL y0 => ... (* Branch of index 0 *)
+         | INR x1
+           case x1 of
+           | INL y1 => ... (* Branch of index 1 *)
+           | INR x2 =>
+             case x2 of
+             | INL y2 => ... (* Branch of index 2 *)
+             | INR y3 => ... (* Branch of index 3 *)
+       ]}
      *)
-    val ids = map (fst o strip_comb o lhs) def_tms
+    fun create_case (j : int) (scrut : term) (tys : hol_type list) : term =
+      let
+        val _ = print_dbg ("list_mk_sum_case: " ^
+                           String.concatWith ", " (map type_to_string tys) ^ "\n")
+      in
+        case tys of
+          [] => failwith "tys is too short"
+        | [ ty ] =>
+          (* Last element: no match to perform *)
+          gen_branch j scrut
+        | ty1 :: tys =>
+          (* Not last: we create a pattern:
+             {[
+               case scrut of
+               | INL pat_var1 => ... (* Branch of index i *)
+               | INR pat_var2 =>
+                 ... (* Generate this term recursively *)
+             ]}
+           *)
+          let
+            (* INL branch *)
+            val after_ty = sumSyntax.list_mk_sum tys
+            val pat_var1 = genvar ty1
+            val pat1 = sumSyntax.mk_inl (pat_var1, after_ty)
+            val br1 = gen_branch j pat_var1
+            (* INR branch *)
+            val pat_var2 = genvar after_ty
+            val pat2 = sumSyntax.mk_inr (pat_var2, ty1)
+            val br2 = create_case (j+1) pat_var2 tys
+            val _ = print_dbg ("list_mk_sum_case: assembling:\n" ^
+                               term_to_string scrut ^ ",\n" ^
+                               "[(" ^ term_to_string pat1 ^ ",\n  " ^ term_to_string br1 ^ "),\n\n" ^
+                               " (" ^ term_to_string pat2 ^ ",\n  " ^ term_to_string br2 ^ ")]\n\n")
+            val case_elems = (scrut, [(pat1, br1), (pat2, br2)])
+            val _ = list_mk_sum_case_case := case_elems
+          in
+            (* Put everything together *)
+            TypeBase.mk_case case_elems
+          end
+      end
+  in
+    create_case 0 scrut tys
+  end
 
-    (* In the definitions, replace the identifiers by new identifiers which use
-       fuel.
+(* Generate a ‘case ... of’ to select the input/output of the ith variant of
+   the param enumeration.
 
-       Ex.:
-       def_fuel_tm = “
-         even___fuel (fuel : nat) (n : int) : result bool =
-           case fuel of 0 => Diverge
-           | SUC fuel' => 
-             if i = 0 then Return T else odd_fuel fuel' (i - 1))”
+   Ex.:
+   ====
+   There are two functions in the group, and we select the input of the function of index 1:
+   {[
+     case x of
+     | INL _ => Fail Failure              (* Input of function of index 0 *)
+     | INR (INL _) => Fail Failure        (* Output of function of index 0 *)
+     | INR (INR (INL y)) => Return y      (* Input of the function of index 1: select this one *)
+     | INR (INR (INR _)) => Fail Failure  (* Output of the function of index 1 *)
+   ]}
+
+   (* Debug *)
+   val tys = [(“:'a”, “:'b”)]
+   val scrut = “x : 'a + 'b”
+   val fi = 0
+   val is_input = true
+
+   val tys = [(“:'a”, “:'b”), (“:'c”, “:'d”)]
+   val scrut = “x : 'a + 'b + 'c + 'd”
+   val fi = 1
+   val is_input = false
+
+   val scrut = mk_var ("x", sumSyntax.list_mk_sum (flatten tys))
+
+   list_mk_case_select scrut tys fi is_input
+ *)
+fun list_mk_case_sum_select (scrut : term) (tys : (hol_type * hol_type) list)
+  (fi : int) (is_input : bool) : term =
+  let
+    (* The index of the element in the enumeration that we will select *)
+    val i = 2 * fi + (if is_input then 0 else 1)
+    (* Flatten the types and numerotate them *)
+    fun flatten ls = List.concat (map (fn (x, y) => [x, y]) ls)
+    val tys = flatten tys
+    (* Get the return type *)
+    val ret_ty = List.nth (tys, i)
+    (* The continuation which will generate the content of the branches *)
+    fun gen_branch j var = if j = i then mk_return var else mk_fail_failure ret_ty
+  in
+    (* Generate the ‘case ... of’ *)
+    list_mk_sum_case scrut tys gen_branch
+  end
+
+(* Generate a ‘case ... of’ to select the input/output of the ith variant of
+   the param enumeration.
+
+   Ex.:
+   ====
+   There are two functions in the group, and we select the input of the function of index 1:
+   {[
+     case x of
+     | Fail e => Fail e
+     | Diverge => Diverge
+     | Return r =>
+       case r of
+       | INL _ => Fail Failure              (* Input of function of index 0 *)
+       | INR (INL _) => Fail Failure        (* Output of function of index 0 *)
+       | INR (INR (INL y)) => Return y      (* Input of the function of index 1: select this one *)
+       | INR (INR (INR _)) => Fail Failure  (* Output of the function of index 1 *)
+   ]}
+ *)
+fun mk_case_select_result_sum (scrut : term) (tys : (hol_type * hol_type) list)
+  (fi : int) (is_input : bool) : term =
+  (* We match over the result, then over the enumeration *)
+  mk_result_case scrut (fn x => list_mk_case_sum_select x tys fi is_input)
+
+(* Generate a body for the fixed-point operator from a quoted group of mutually
+   recursive definitions.
+
+   See TODO for detailed explanations: from the quoted equations for ‘nth’
+   (or for [‘even’, ‘odd’]) we generate the body ‘nth_body’ (or ‘even_odd_body’,
+   respectively).
+ *)
+fun mk_body (fnames : string list) (in_out_tys : (hol_type * hol_type) list)
+  (def_tms : term list) : term =
+  let
+    val fnames_set = Redblackset.fromList String.compare fnames
+
+    (* Compute a map from function name to function index *)
+    val fnames_map = Redblackmap.fromList String.compare
+      (map (fn (x, y) => (y, x)) (enumerate fnames))
+
+    (* Compute the input/output type, that we dub the "parameter type" *)
+    fun flatten ls = List.concat (map (fn (x, y) => [x, y]) ls)
+    val param_type = sumSyntax.list_mk_sum (flatten in_out_tys)
+
+    (* Introduce a variable for the confinuation *)
+    val fcont = genvar (param_type --> mk_result param_type)
+
+    (* In the function equations, replace all the recursive calls with calls to the continuation.
+
+       When replacing a recursive call, we have to do two things:
+       - we need to inject the input parameters into the parameter type
+         Ex.:
+         - ‘nth tl i’ becomes ‘f (INL (tl, i))’ where ‘f’ is the continuation
+         - ‘even i’ becomes ‘f (INL i)’ where ‘f’ is the continuation
+       - we need to wrap the the call to the continuation into a ‘case ... of’
+         to extract its output (we need to make sure that the transformation
+         preserves the type of the expression!)
+         Ex.: ‘nth tl i’ becomes:
+         {[
+           case f (INL (tl, i)) of
+           | Fail e => Fail e
+           | Diverge => Diverge
+           | Return r =>
+             case r of
+             | INL _ => Fail Failure
+             | INR x => Return (INR x)
+         ]}
      *)
-     val names = map ((fn s => s ^ fuel_def_suffix) o fst o dest_var) ids
-     val index = get_smallest_unique_id_for_names names
-     fun mk_fuel_id (id : term) : term =
+     (* For debugging *)
+     val replace_rec_calls_rec_call_tm = ref “T”
+     fun replace_rec_calls (fnames_set : string Redblackset.set) (tm : term) : term =
        let
-         val (id_str, ty) = dest_var id
-         (* Note: we use symbols forbidden in the generation of code to
-            prevent name collisions *)
-         val fuel_id_str = id_str ^ fuel_def_suffix ^ index
-         val fuel_id = mk_var (fuel_id_str, num_ty --> ty)
-       in fuel_id end
-     val fuel_ids = map mk_fuel_id ids
-
-     val fuel_ids_with_fuel0 = map (fn id => mk_comb (id, fuel_var0)) fuel_ids
-     val fuel_ids_with_fuel1 = map (fn id => mk_comb (id, fuel_var1)) fuel_ids
-
-     (* Recurse through the terms and replace the calls *)
-     val rwr_thms0 = map (ASSUME o mk_eq) (zip ids fuel_ids_with_fuel0)
-     val rwr_thms1 = map (ASSUME o mk_eq) (zip ids fuel_ids_with_fuel1)
-
-     fun mk_fuel_tm (def_tm : term) : term =
-       let
-         val (tm0, tm1) = dest_eq def_tm
-         val tm0 = (rhs o concl o (PURE_REWRITE_CONV rwr_thms0)) tm0
-         val tm1 = (rhs o concl o (PURE_REWRITE_CONV rwr_thms1)) tm1
-       in mk_eq (tm0, tm1) end
-     val fuel_tms = map mk_fuel_tm def_tms
-
-     (* Add the case over the fuel *)
-     fun add_fuel_case (tm : term) : term =
-       let
-         val (f, body) = dest_eq tm
-         (* Create the “Diverge” term with the proper type *)
-         val body_ty = type_of body
-         val return_ty =
-           case (snd o dest_type) body_ty of [ty] => ty
-           | _ => failwith "unexpected"
-         val diverge_tm = mk_diverge_tm return_ty
-         (* Create the “SUC fuel” term *)
-         val suc_tm = mk_comb (num_suc_tm, fuel_var1)
-         val fuel_tm =
-           TypeBase.mk_case (fuel_var0, [(num_zero_tm, diverge_tm), (suc_tm, body)])
-       in mk_eq (f, fuel_tm) end
-     val fuel_tms = map add_fuel_case fuel_tms
-
-     (* Define the auxiliary definitions which use fuel *)
-     val fuel_defs_conj = list_mk_conj fuel_tms
-     (* The definition name *)
-     val def_name = (fst o dest_var o hd) fuel_ids
-     (* The tactic to prove the termination *)
-     val rty = ref “:bool” (* This is useful for debugging *)
-     fun prove_termination_tac (asms, g) =
-       let
-         val r_tm = (fst o dest_exists) g
-         val _ = rty := type_of r_tm
-         val ty = (hd o snd o dest_type) (!rty)
-         val m_tm = mk_termination_measure_from_ty ty
+         val _ = print_dbg ("replace_rec_calls: original expression:\n" ^
+                            term_to_string tm ^ "\n\n")
+         val ntm =
+           case dest_term tm of
+             VAR (name, ty) =>
+             (* Check that this is not one of the functions in the group - remark:
+                we could handle that by introducing lambdas.
+              *)
+             if Redblackset.member (fnames_set, name)
+             then failwith ("mk_body: not well-formed definition: found " ^ name ^
+                            " in an improper position")
+             else tm
+           | CONST _ => tm
+           | LAMB (x, tm) =>
+             let
+               (* The variable might shadow one of the functions *)
+               val fnames_set = Redblackset.delete (fnames_set, (fst o dest_var) x)
+               (* Update the term in the lambda *)
+               val tm = replace_rec_calls fnames_set tm
+             in
+               (* Reconstruct *)
+               mk_abs (x, tm)
+             end
+           | COMB (_, _) =>
+             let
+               (* Completely destruct the application, check if this is a recursive call *)
+               val (app, args) = strip_comb tm
+               val is_rec_call = Redblackset.member (fnames_set, (fst o dest_var) app)
+                 handle HOL_ERR _ => false
+               (* Whatever the case, apply the transformation to all the inputs *)
+               val args = map (replace_rec_calls fnames_set) args
+             in
+               (* If this is not a recursive call: apply the transformation to all the
+                  terms. Otherwise, replace. *)
+               if not is_rec_call then list_mk_comb (replace_rec_calls fnames_set app, args)
+               else
+                 (* Rec call: replace *)
+                 let
+                   val _ = replace_rec_calls_rec_call_tm := tm
+                   (* First, find the index of the function *)
+                   val fname = (fst o dest_var) app
+                   val fi = Redblackmap.find (fnames_map, fname)
+                   (* Inject the input values into the param type *)
+                   val input = pairSyntax.list_mk_pair args
+                   val input = inject_in_param_sum in_out_tys fi true input
+                   (* Create the recursive call *)
+                   val call = mk_comb (fcont, input)
+                   (* Wrap the call into a ‘case ... of’ to extract the output *)
+                   val call = mk_case_select_result_sum call in_out_tys fi false
+                 in
+                   (* Return *)
+                   call
+                 end
+             end
+         val _ = print_dbg ("replace_rec_calls: new expression:\n" ^ term_to_string ntm ^ "\n\n")
        in
-         WF_REL_TAC ‘^m_tm’ (asms, g)
+         ntm
        end
+       handle HOL_ERR e =>
+         let
+           val _ = print_dbg ("replace_rec_calls: failed on:\n" ^ term_to_string tm ^ "\n\n")
+         in
+           raise (HOL_ERR e)
+         end
+     fun replace_rec_calls_in_eq (eq : term) : term =
+       let
+         val (l, r) = dest_eq eq
+       in
+         mk_eq (l, replace_rec_calls fnames_set r)
+       end
+     val def_tms_with_fcont = map replace_rec_calls_in_eq def_tms
 
-     (* Define the fuel definitions *)
-     (*
-       val temp_def = Hol_defn def_name ‘^fuel_defs_conj’
-       Defn.tgoal temp_def
-     *)
-     val fuel_defs = tDefine def_name ‘^fuel_defs_conj’ prove_termination_tac
-   in
-     CONJUNCTS fuel_defs
-   end
+     (* Wrap all the function bodies to inject their result into the param type.
 
-(*
-val (fuel_tms, fuel_defs) = mk_fuel_defs def_tms
-val fuel_def_tms = map (snd o strip_forall) ((strip_conj o concl) fuel_defs)
-val (def_tm, fuel_def_tm) = hd (zip def_tms fuel_def_tms)
-*)
+        We collect the function inputs at the same time, because they will be
+        grouped into a tuple that we will have to deconstruct.
+      *)
+     fun inject_body_to_enums (i : int, def_eq : term) : term list * term =
+       let
+         val (l, body) = dest_eq def_eq
+         val (_, args) = strip_comb l
+         (* We have the deconstruct the result, then, in the ‘Return’ branch,
+            properly wrap the returned value *)
+         val body = mk_result_case body (fn x => mk_return (inject_in_param_sum in_out_tys i false x))
+       in
+         (args, body)
+       end
+     val def_tms_inject = map inject_body_to_enums (enumerate def_tms_with_fcont)
 
-fun mk_is_diverge_tm (fuel_tm : term) : term =
-  case snd (dest_type (type_of fuel_tm)) of
-    [ret_ty] => mk_comb (inst [alpha_tyvar |-> ret_ty] is_diverge_tm, fuel_tm)
-   | _ => failwith "mk_is_diverge_tm: unexpected"
+     (* Currify the body inputs.
 
-fun mk_fuel_predicate_defs (def_tm, fuel_def_tm) : thm =
-  let
-    (* From [even i] create the term [even_P i n], where [n] is the fuel *)
-    val (id, args) = (strip_comb o lhs) def_tm
-    val (id_str, id_ty) = dest_var id
-    val (tys, ret_ty) = strip_arrows id_ty
-    val tys = append tys [num_ty]
-    val pred_ty = list_mk_arrow tys bool_ty
-    val pred_id = mk_var (id_str ^ fuel_predicate_suffix, pred_ty)
-    val pred_tm = list_mk_comb (pred_id, append args [fuel_var])
+        For instance, if the body has inputs: ‘x’, ‘y’; we return the following:
+        {[
+          (‘z’, ‘case z of (x, y) => ... (* body *) ’)
+        ]}
+        where ‘z’ is fresh.
 
-    (* Create the term ~is_diverge (even_fuel n i) *)
-    val fuel_tm = lhs fuel_def_tm
-    val not_is_diverge_tm = mk_neg (mk_is_diverge_tm fuel_tm)
+        We return: (curried input, body).
 
-    (* Create the term: even_P i n = ~(is_diverge (even_fuel n i) *)
-    val pred_def_tm = mk_eq (pred_tm, not_is_diverge_tm)
+        (* Debug *)
+        val body = “(x:'a, y:'b, z:'c)”
+        val args = [“x:'a”, “y:'b”, “z:'c”]
+        currify_body_inputs (args, body)
+      *)
+     fun currify_body_inputs (args : term list, body : term) : term * term =
+       let
+         fun mk_curry (args : term list) (body : term) : term * term =
+           case args of
+             [] => failwith "no inputs"
+           | [x] => (x, body)
+           | x1 :: args =>
+             let
+               val (x2, body) = mk_curry args body
+               val scrut = genvar (pairSyntax.list_mk_prod (map type_of (x1 :: args)))
+               val pat = pairSyntax.mk_pair (x1, x2)
+               val br = body
+             in
+               (scrut, TypeBase.mk_case (scrut, [(pat, br)]))
+             end
+       in
+         mk_curry args body
+       end
+     val def_tms_currified = map currify_body_inputs def_tms_inject
+
+     (* Group all the functions into a single body, with an outer ‘case .. of’
+        which selects the appropriate body depending on the input *)
+     val param_ty = sumSyntax.list_mk_sum (flatten in_out_tys)
+     val input = genvar param_ty
+     fun mk_mut_rec_body_branch (i : int) (patvar : term) : term =
+       (* Case disjunction on whether the branch is for an input value (in
+          which case we call the proper body) or an output value (in which
+          case we return ‘Fail ...’ *)
+       if i mod 2 = 0 then
+         let
+           val fi = i div 2
+           val (x, def_tm) = List.nth (def_tms_currified, fi)
+           (* The variable in the pattern and the variable expected by the
+              body may not be the same: we introduce a let binding *)
+           val def_tm = mk_let (mk_abs (x, def_tm), patvar)
+         in
+           def_tm
+         end
+       else
+         (* Output value: fail *)
+         mk_fail_failure param_ty
+     val mut_rec_body = list_mk_sum_case input (flatten in_out_tys) mk_mut_rec_body_branch
+
+
+     (* Abstract away the parameters to produce the final body of the fixed point *)
+     val mut_rec_body = list_mk_abs ([fcont, input], mut_rec_body)
   in
-    (* Create the definition *)
-    Define ‘^pred_def_tm’
+    mut_rec_body
   end
 
-(*
-val (def_tm, fuel_def_tm) = hd (zip def_tms fuel_def_tms)
+(*=============================================================================*
+ *
+ * Prove that the body satisfies the validity condition
+ *
+ * ============================================================================*)
 
-val pred_defs = map mk_fuel_predicate_defs (zip def_tms fuel_def_tms)
-*)
+(* Tactic to prove that a body is valid: perform one step. *)
+fun prove_body_is_valid_tac_step (asms, g) =
+  let
+    (* The goal has the shape:
+       {[
+         (∀g h. ... g x = ... h x) ∨
+         ∃h y. is_valid_fp_body n h ∧ ∀g. ... g x = ... od
+       ]}   
+     *)
+    (* Retrieve the scrutinee in the goal (‘x’).
+       There are two cases:
+       - either the function has the shape:
+         {[
+           (λ(y,z). ...) x
+         ]}
+         in which case we need to destruct ‘x’
+       - or we have a normal ‘case ... of’
+     *)
+    val body = (lhs o snd o strip_forall o fst o dest_disj) g
+    val scrut =
+      let
+        val (app, x) = dest_comb body
+        val (app, _) = dest_comb app
+        val {Name=name, Thy=thy, Ty = _ } = dest_thy_const app
+      in
+        if thy = "pair" andalso name = "UNCURRY" then x else failwith "not a curried argument"
+      end
+      handle HOL_ERR _ => strip_all_cases_get_scrutinee body
+    (* Retrieve the first quantified continuations from the goal (‘g’) *)
+    val qc = (hd o fst o strip_forall o fst o dest_disj) g
+    (* Check if the scrutinee is a recursive call *)
+    val (scrut_app, _) = strip_comb scrut
+    val _ = print_dbg ("prove_body_is_valid_step: Scrutinee: " ^ term_to_string scrut ^ "\n")
+    (* For the recursive calls: *)
+    fun step_rec () =
+      let
+        val _ = print_dbg ("prove_body_is_valid_step: rec call\n")
+        (* We need to instantiate the ‘h’ existantially quantified function *)
+        (* First, retrieve the body of the function: it is given by the ‘Return’ branch *)
+        val (_, _, branches) = TypeBase.dest_case body
+        (* Find the branch corresponding to the return *)
+        val ret_branch = List.find (fn (pat, _) =>
+          let
+            val {Name=name, Thy=thy, Ty = _ } = (dest_thy_const o fst o strip_comb) pat
+          in
+            thy = "primitives" andalso name = "Return"
+          end) branches
+        val var = (hd o snd o strip_comb o fst o valOf) ret_branch
+        val br = (snd o valOf) ret_branch
+        (* Abstract away the input variable introduced by the pattern and the continuation ‘g’ *)
+        val h = list_mk_abs ([qc, var], br)
+        val _ = print_dbg ("prove_body_is_valid_step: h: " ^ term_to_string h ^ "\n")
+        (* Retrieve the input parameter ‘x’ *)
+        val input = (snd o dest_comb) scrut
+        val _ = print_dbg ("prove_body_is_valid_step: y: " ^ term_to_string input ^ "\n")
+      in
+        ((* Choose the right possibility (this is a recursive call) *)
+         disj2_tac >>
+         (* Instantiate the quantifiers *)
+         qexists ‘^h’ >>
+         qexists ‘^input’ >>
+         (* Unfold the predicate once *)
+         pure_once_rewrite_tac [is_valid_fp_body_def] >>
+         (* We have two subgoals:
+            - we have to prove that ‘h’ is valid
+            - we have to finish the proof of validity for the current body
+          *)
+         conj_tac >> fs [case_result_switch_eq])
+      end
+  in
+    (* If recursive call: special treatment. Otherwise, we do a simple disjunction *)
+    (if term_eq scrut_app qc then step_rec ()
+     else (Cases_on ‘^scrut’ >> fs [case_result_switch_eq])) (asms, g)
+  end
+
+(* Tactic to prove that a body is valid *)
+fun prove_body_is_valid_tac (body_def : thm option) : tactic =
+  let val body_def_thm = case body_def of SOME th => [th] | NONE => []
+  in
+    pure_once_rewrite_tac [is_valid_fp_body_def] >> gen_tac >>
+    (* Expand *)
+    fs body_def_thm >>
+    fs [bind_def, case_result_switch_eq] >>
+    (* Explore the body *)
+    rpt prove_body_is_valid_tac_step
+  end
+
+(* Prove that a body satisfies the validity condition of the fixed point *)
+fun prove_body_is_valid (body : term) : thm =
+  let
+    (* Explore the body and count the number of occurrences of nested recursive
+       calls so that we can properly instantiate the ‘N’ argument of ‘is_valid_fp_body’.
+
+       We first retrieve the name of the continuation parameter.
+       Rem.: we generated fresh names so that, for instance, the continuation name
+       doesn't collide with other names. Because of this, we don't need to look for
+       collisions when exploring the body (and in the worst case, we would cound
+       an overapproximation of the number of recursive calls, which is perfectly
+       valid).
+     *)
+    val fcont = (hd o fst o strip_abs) body
+    val fcont_name = (fst o dest_var) fcont
+    fun max x y = if x > y then x else y
+    fun count_body_rec_calls (body : term) : int =
+      case dest_term body of
+        VAR (name, _) => if name = fcont_name then 1 else 0
+      | CONST _ => 0
+      | COMB (x, y) => max (count_body_rec_calls x) (count_body_rec_calls y)
+      | LAMB (_, x) => count_body_rec_calls x
+    val num_rec_calls = count_body_rec_calls body
+
+    (* Generate the term ‘SUC (SUC ... (SUC n))’ where ‘n’ is a fresh variable.
+
+       Remark: we first prove ‘is_valid_fp_body (SUC ... n) body’ then substitue
+       ‘n’ with ‘0’ to prevent the quantity from being rewritten to a bit
+       representation, which would prevent unfolding of the ‘is_valid_fp_body’.
+     *)
+    val nvar = genvar num_ty
+    (* Rem.: we stack num_rec_calls + 1 occurrences of ‘SUC’ (and the + 1 is important) *)
+    fun mk_n i = if i = 0 then mk_suc nvar else mk_suc (mk_n (i-1))
+    val n_tm = mk_n num_rec_calls
+
+    (* Generate the lemma statement *)
+    val is_valid_tm = list_mk_icomb (is_valid_fp_body_tm, [n_tm, body])
+    val is_valid_thm = prove (is_valid_tm, prove_body_is_valid_tac NONE)
+
+    (* Replace ‘nvar’ with ‘0’ *)
+    val is_valid_thm = INST [nvar |-> zero_num_tm] is_valid_thm
+  in
+    is_valid_thm
+  end
+
+(*=============================================================================*
+ *
+ * Generate the definitions with the fixed-point operator
+ *
+ * ============================================================================*)
+
+(* Generate the raw definitions by using the grouped definition body and the
+   fixed point operator *)
+fun mk_raw_defs (in_out_tys : (hol_type * hol_type) list)
+  (def_tms : term list) (body_is_valid : thm) : thm list =
+  let
+    (* Retrieve the body *)
+    val body = (List.last o snd o strip_comb o concl) body_is_valid
+
+    (* Create the term ‘fix body’ *)
+    val fixed_body = mk_icomb (fix_tm, body)
+
+    (* For every function in the group, generate the equation that we will
+       use as definition. In particular:
+       - add the properly injected input ‘x’ to ‘fix body’ (ex.: for ‘nth ls i’
+         we add the input ‘INL (ls, i)’)
+       - wrap ‘fix body x’ into a case disjunction to extract the relevant output
+
+       For instance, in the case of ‘nth ls i’:
+       {[
+         nth (ls : 't list_t) (i : u32) =
+           case fix nth_body (INL (ls, i)) of
+           | Fail e => Fail e
+           | Diverge => Diverge
+           | Return r =>
+             case r of
+             | INL _ => Fail Failure
+             | INR x => Return x
+       ]}
+     *)
+    fun mk_def_eq (i : int, def_tm : term) : term =
+      let
+        (* Retrieve the lhs of the original definition equation, and in
+           particular the inputs *)
+        val def_lhs = lhs def_tm
+        val args = (snd o strip_comb) def_lhs
+
+        (* Inject the inputs into the param type *)
+        val input = pairSyntax.list_mk_pair args
+        val input = inject_in_param_sum in_out_tys i true input
+
+        (* Compose*)
+        val def_rhs = mk_comb (fixed_body, input)
+
+        (* Wrap in the case disjunction *)
+        val def_rhs = mk_case_select_result_sum def_rhs in_out_tys i false
+
+        (* Create the equation *)
+        val def_eq_tm = mk_eq (def_lhs, def_rhs)
+      in
+        def_eq_tm
+      end
+    val raw_def_tms = map mk_def_eq (enumerate def_tms)
+
+    (* Generate the definitions *)
+    val raw_defs = map (fn tm => Define ‘^tm’) raw_def_tms
+  in
+    raw_defs
+  end
+
+(*=============================================================================*
+ *
+ * Prove that the definitions satisfy the target equations
+ *
+ * ============================================================================*)
 
 (* Tactic which makes progress in a proof by making a case disjunction (we use
    this to explore all the paths in a function body). *)
 fun case_progress (asms, g) =
   let
     val scrut = (strip_all_cases_get_scrutinee o lhs) g
-  in Cases_on ‘^scrut’ (asms, g) end  
+  in Cases_on ‘^scrut’ (asms, g) end
 
-(* Prove the fuel monotonicity properties.
-
-   We want to prove a theorem of the shape:
-   {[
-     !n m.
-       (!i. n <= m ==> even___P i n ==> even___fuel n i = even___fuel m i) /\
-       (!i. n <= m ==> odd___P i n ==> odd___fuel n i = odd___fuel m i)
-   ]}
-*)
-fun prove_fuel_mono (pred_defs : thm list) (fuel_defs : thm list) : thm =
+(* Prove the final equation, that we will use as definition. *)
+fun prove_def_eq_tac
+  (current_raw_def : thm) (all_raw_defs : thm list) (is_valid : thm)
+  (body_def : thm option) : tactic =
   let
-    val pred_tms = map (lhs o snd o strip_forall o concl) pred_defs
-    val fuel_tms = map (lhs o snd o strip_forall o concl) fuel_defs
-    val pred_fuel_tms = zip pred_tms fuel_tms
-    (* Create a set containing the names of all the functions in the recursive group *)
-    val rec_fun_set =
-      Redblackset.fromList const_name_compare (map get_fun_name_from_app fuel_tms)
-    (* Small tactic which rewrites the occurrences of recursive calls *)
-    fun rewrite_rec_call (asms, g) =
-      let
-        val scrut = (strip_all_cases_get_scrutinee o lhs) g
-        val fun_id = get_fun_name_from_app scrut (* This can fail *)
-      in
-        (* Check if the function is part of the group we are considering *)
-        if Redblackset.member (rec_fun_set, fun_id) then
-          let
-             (* Yes: use the induction hypothesis *)
-             fun apply_ind_hyp (ind_th : thm) : tactic =
-               let
-                  val th = SPEC_ALL ind_th
-                  val th_pat = (lhs o snd o strip_imp o concl) th
-                  val (var_s, ty_s) = match_term th_pat scrut
-                  (* Note that in practice the type instantiation should be empty *)
-                  val th = INST var_s (INST_TYPE ty_s th)
-               in
-                 assume_tac th
-               end
-          in
-            (last_assum apply_ind_hyp >> fs []) (asms, g)
-          end
-        else all_tac (asms, g)
-      end
-      handle HOL_ERR _ => all_tac (asms, g)
-    (* Generate terms of the shape:
-       !i. n <= m ==> even___P i n ==> even___fuel n i = even___fuel m i
-     *)
-    fun mk_fuel_eq_tm (pred_tm, fuel_tm) : term =
-      let
-        (* Retrieve the variables which are not the fuel - for the quantifiers *)
-        val vars = (tl o snd o strip_comb) fuel_tm
-        (* Introduce the fuel term which uses “m” *)
-        val m_fuel_tm = subst [fuel_var0 |-> fuel_var1] fuel_tm
-        (* Introduce the equality *)
-        val fuel_eq_tm = mk_eq (fuel_tm, m_fuel_tm)
-        (* Introduce the implication with the _P pred *)
-        val fuel_eq_tm = mk_imp (pred_tm, fuel_eq_tm)
-        (* Introduce the “n <= m ==> ...” implication *)
-        val fuel_eq_tm = mk_imp (fuel_vars_le, fuel_eq_tm)
-        (* Quantify *)
-        val fuel_eq_tm = list_mk_forall (vars, fuel_eq_tm)
-      in
-        fuel_eq_tm
-      end
-     val fuel_eq_tms = map mk_fuel_eq_tm pred_fuel_tms
-     (* Create the conjunction *)
-     val fuel_eq_tms = list_mk_conj fuel_eq_tms
-     (* Qantify over the fuels *)
-     val fuel_eq_tms = list_mk_forall ([fuel_var0, fuel_var1], fuel_eq_tms)
-     (* The tactics for the proof *)
-     val prove_tac =
-       Induct_on ‘^fuel_var0’ >-(
-         (* The ___P predicates are false: n is 0 *)
-         fs pred_defs >>
-         fs [is_diverge_def] >>
-         pure_once_rewrite_tac fuel_defs >> fs []) >>
-       (* Introduce n *)
-       gen_tac >>
-       (* Introduce m *)
-       Cases_on ‘^fuel_var1’ >-(
-         (* Contradiction: SUC n < 0 *)
-         rw [] >> exfalso >> int_tac) >>
-       fs pred_defs >>
-       fs [is_diverge_def] >>
-       pure_once_rewrite_tac fuel_defs >> fs [bind_def] >>
-       (* Introduce in the context *)
-       rpt gen_tac >>
-       (* Split the goals - note that we prove one big goal for all the functions at once *)
-       rpt strip_tac >>
-       (* Instantiate the assumption: !m. n <= m ==> ~(...)
-          with the proper m.
-        *)
-       last_x_assum imp_res_tac >>
-       (* Make sure the induction hypothesis is always the last assumption *)
-       last_x_assum assume_tac >>
-       (* Split the goals *)
-       rpt strip_tac >> fs [case_result_same_eq] >>
-       (* Explore all the paths *)
-       rpt (rewrite_rec_call >> case_progress >> fs [case_result_same_eq])
-   in
-     (* Prove *)
-     save_goal_and_prove (fuel_eq_tms, prove_tac)
-   end
-
-(*
-val fuel_mono_thm = prove_fuel_mono pred_defs fuel_defs
-
-set_goal ([], fuel_eq_tms)
-*)
-
-(* Prove the property about the least upper bound.
-
-   We want to prove theorems of the shape:
-   {[
-     (!n i. $LEAST (even___P i) <= n ==> even___fuel n i = even___fuel ($LEAST (even___P i)) i)
-   ]}
-   {[
-     (!n i. $LEAST (odd___P i) <= n ==> odd___fuel n i = odd___fuel ($LEAST (odd___P i)) i)
-   ]}
-
-   TODO: merge with other functions? (prove_pred_imp_fuel_eq_raw_thms)
-*)
-fun prove_least_fuel_mono (pred_defs : thm list) (fuel_mono_thm : thm) : thm list =
-  let
-    val thl = (CONJUNCTS o SPECL [fuel_var0, fuel_var1]) fuel_mono_thm
-    fun mk_least_fuel_thm (pred_def, mono_thm) : thm =
-      let
-        (* Retrieve the predicate, without the fuel *)
-        val pred_tm = (lhs o snd o strip_forall o concl) pred_def
-        val (pred_tm, args) = strip_comb pred_tm
-        val args = rev (tl (rev args))
-        val pred_tm = list_mk_comb (pred_tm, args)
-        (* Add $LEAST *)
-        val least_pred_tm = mk_comb (least_tm, pred_tm)
-        (* Specialize all *)
-        val vars = (fst o strip_forall o concl) mono_thm
-        val th = SPECL vars mono_thm
-        (* Substitute in the mono theorem *)
-        val th = INST [fuel_var0 |-> least_pred_tm] th
-        (* Symmetrize the equality *)
-        val th = PURE_ONCE_REWRITE_RULE [EQ_SYM_EQ] th
-        (* Quantify *)
-        val th = GENL (fuel_var1 :: vars) th
-      in
-        th
-      end
+    val body_def_thm = case body_def of SOME th => [th] | NONE => []
   in
-    map mk_least_fuel_thm (zip pred_defs thl)
+    rpt gen_tac >>
+    (* Expand the definition *)
+    pure_once_rewrite_tac [current_raw_def] >>
+    (* Use the fixed-point equality *)
+    pure_once_rewrite_left_tac [HO_MATCH_MP fix_fixed_eq is_valid] >>
+    (* Expand the body definition *)
+    pure_rewrite_tac body_def_thm >>
+    (* Expand all the definitions from the group *)
+    pure_rewrite_tac all_raw_defs >>
+    (* Explore all the paths - maybe we can be smarter, but this is fast and really easy *)
+    fs [bind_def] >>
+    rpt (case_progress >> fs [])
   end
 
-(*
-val (pred_def, mono_thm) = hd (zip pred_defs thl)
-*)
-
-(* Prove theorems of the shape:
-
-   {[
-     !n i. even___P i n ==> $LEAST (even___P i) <= n
-   ]}
-
-   TODO: merge with other functions? (prove_pred_imp_fuel_eq_raw_thms)
- *)
-fun prove_least_pred_thms (pred_defs : thm list) : thm list =
+(* Prove the final equations that we will give to the user as definitions *)
+fun prove_def_eqs (body_is_valid : thm) (def_tms : term list) (raw_defs : thm list) : thm list=
   let
-    fun prove_least_pred_thm (pred_def : thm) : thm =
+    val defs_tgt_raw = zip def_tms raw_defs
+    (* Substitute the function variables with the constants introduced in the raw
+       definitions *)
+    fun compute_fsubst (def_tm, raw_def) : {redex: term, residue: term} =
       let
-        val pred_tm = (lhs o snd o strip_forall o concl) pred_def
-        val (pred_no_fuel_tm, args) = strip_comb pred_tm
-        val args = rev (tl (rev args))
-        val pred_no_fuel_tm = list_mk_comb (pred_no_fuel_tm, args)
-        (* Make the “$LEAST (even___P i)” term *)
-        val least_pred_tm = mk_comb (least_tm, pred_no_fuel_tm)
-        (* Make the inequality *)
-        val tm = list_mk_comb (le_tm, [least_pred_tm, fuel_var0])
-        (* Add the implication *)
-        val tm = mk_imp (pred_tm, tm)
-        (* Quantify *)
-        val tm = list_mk_forall (args, tm)
-        val tm = mk_forall (fuel_var0, tm)
+        val (fvar, _) = (strip_comb o lhs) def_tm
+        val fconst = (fst o strip_comb o lhs o snd o strip_forall o concl) raw_def
+      in
+        (fvar |-> fconst)
+      end
+    val fsubst = map compute_fsubst defs_tgt_raw
+    val defs_tgt_raw = map (fn (x, y) => (subst fsubst x, y)) defs_tgt_raw
+
+    fun prove_def_eq (def_tm, raw_def) : thm =
+      let
+        (* Quantify the parameters *)
+        val (_, params) = (strip_comb o lhs) def_tm
+        val def_eq_tm = list_mk_forall (params, def_tm)
         (* Prove *)
-        val prove_tac =
-          rpt gen_tac >>
-          disch_tac >>
-          (* Use the "fundamental" property about $LEAST *)
-          qspec_assume ‘^pred_no_fuel_tm’ whileTheory.LEAST_EXISTS_IMP >>
-          (* Prove the premise *)
-          pop_assum sg_premise_tac >- (exists_tac fuel_var0 >> fs []) >>
-          rw [] >>
-          (* Finish the proof by contraposition *)
-          spose_not_then assume_tac >>
-          fs [not_le_eq_gt]
+        val def_eq = prove (def_eq_tm, prove_def_eq_tac raw_def raw_defs body_is_valid NONE)
       in
-        save_goal_and_prove (tm, prove_tac)
+        def_eq
       end
+    val def_eqs = map prove_def_eq defs_tgt_raw
   in
-    map prove_least_pred_thm pred_defs
+    def_eqs
   end
 
+(*=============================================================================*
+ *
+ * The final DefineDiv function
+ *
+ * ============================================================================*)
 
-(*
-val least_pred_thms = prove_least_pred_thms pred_defs
-
-val least_pred_thm = hd least_pred_thms
-*)
-
-(* Prove theorems of the shape:
-
-   {[
-     !n i. even___P i n ==> even___P i ($LEAST (even___P i))
-   ]}
-*)
-fun prove_pred_n_imp_pred_least_thms (pred_defs : thm list) : thm list =
-  let
-    fun prove_pred_n_imp_pred_least (pred_def : thm) : thm =
-      let
-        val pred_tm = (lhs o snd o strip_forall o concl) pred_def
-        val (pred_no_fuel_tm, args) = strip_comb pred_tm
-        val args = rev (tl (rev args))
-        val pred_no_fuel_tm = list_mk_comb (pred_no_fuel_tm, args)
-        (* Make the “$LEAST (even___P i)” term *)
-        val least_pred_tm = mk_comb (least_tm, pred_no_fuel_tm)
-        (* Make the “even___P i ($LEAST (even___P i))” *)
-        val tm = subst [fuel_var0 |-> least_pred_tm] pred_tm
-        (* Add the implication *)
-        val tm = mk_imp (pred_tm, tm)
-        (* Quantify *)
-        val tm = list_mk_forall (args, tm)
-        val tm = mk_forall (fuel_var0, tm)
-        (* The proof tactic *)
-        val prove_tac =
-          rpt gen_tac >>
-          disch_tac >>
-          (* Use the "fundamental" property about $LEAST *)
-          qspec_assume ‘^pred_no_fuel_tm’ whileTheory.LEAST_EXISTS_IMP >>
-          (* Prove the premise *)
-          pop_assum sg_premise_tac >- (exists_tac fuel_var0 >> fs []) >>
-          rw []
-      in
-        save_goal_and_prove (tm, prove_tac)
-      end
-  in
-    map prove_pred_n_imp_pred_least pred_defs
-  end
-
-(*
-val (pred_def, mono_thm) = hd (zip pred_defs thl)
-val least_fuel_mono_thms = prove_least_fuel_mono pred_defs fuel_defs fuel_mono_thm
-
-val least_fuel_mono_thm = hd least_fuel_mono_thms
-*)
-
-(* Define the "raw" definitions:
-
-   {[
-     even i = if (?n. even___P i n) then even___P ($LEAST (even___P i)) i else Diverge
-   ]}
- *)
-fun define_raw_defs (def_tms : term list) (pred_defs : thm list) (fuel_defs : thm list) : thm list =
-  let
-    fun define_raw_def (def_tm, (pred_def, fuel_def)) : thm =
-      let
-        val app = lhs def_tm
-        val pred_tm = (lhs o snd o strip_forall o concl) pred_def
-        (* Make the “?n. even___P i n” term *)
-        val exists_fuel_tm = mk_exists (fuel_var0, pred_tm)
-        (* Make the “even___fuel ($LEAST (even___P i)) i” term *)
-        val fuel_tm = (lhs o snd o strip_forall o concl) fuel_def
-        val (pred_tm, args) = strip_comb pred_tm
-        val args = rev (tl (rev args))
-        val pred_tm = list_mk_comb (pred_tm, args)
-        val least_pred_tm = mk_comb (least_tm, pred_tm)
-        val fuel_tm = subst [fuel_var0 |-> least_pred_tm] fuel_tm
-        (* Create the Diverge term *)
-        val ret_ty = (hd o snd o dest_type) (type_of app)
-        (* Create the “if then else” *)
-        val body = TypeBase.mk_case (exists_fuel_tm, [(true_tm, fuel_tm), (false_tm, mk_diverge_tm ret_ty)])
-        (* *)
-        val raw_def_tm = mk_eq (app, body)
-      in
-        Define ‘^raw_def_tm’
-      end
-  in
-    map define_raw_def (zip def_tms (zip pred_defs fuel_defs))
-  end
-
-(*
-val raw_defs = define_raw_defs def_tms pred_defs fuel_defs
- *)
-
-(* Prove theorems of the shape:
-
-   !n i. even___P i n ==> even___fuel n i = even i
- *)
-fun prove_pred_imp_fuel_eq_raw_defs
-  (pred_defs : thm list)
-  (fuel_def_tms : term list)
-  (least_fuel_mono_thms : thm list)
-  (least_pred_thms : thm list)
-  (pred_n_imp_pred_least_thms : thm list)
-  (raw_defs : thm list) :
-  thm list =
-  let
-    fun prove_thm (pred_def,
-                   (fuel_def_tm,
-                    (least_fuel_mono_thm,
-                     (least_pred_thm,
-                      (pred_n_imp_pred_least_thm, raw_def))))) : thm =
-      let
-        (* Generate: “even___P i n” *)
-        val pred_tm = (lhs o snd o strip_forall o concl) pred_def
-        val (pred_no_fuel_tm, args) = strip_comb pred_tm
-        val args = rev (tl (rev args))
-        (* Generate: “even___fuel n i” *)
-        val fuel_tm = lhs fuel_def_tm
-        (* Generate: “even i” *)
-        val raw_def_tm = (lhs o snd o strip_forall o concl) raw_def
-        (* Generate: “even___fuel n i = even i” *)
-        val tm = mk_eq (fuel_tm, raw_def_tm)
-        (* Add the implication *)
-        val tm = mk_imp (pred_tm, tm)
-        (* Quantify *)
-        val tm = list_mk_forall (args, tm)
-        val tm = mk_forall (fuel_var0, tm)
-        (* Prove *)
-        val prove_tac =
-          rpt gen_tac >>
-          strip_tac >>
-          fs raw_defs >>
-          (* Case on ‘?n. even___P i n’ *)
-          CASE_TAC >> fs [] >>
-          (* Use the monotonicity property *)
-          irule least_fuel_mono_thm >>
-          imp_res_tac pred_n_imp_pred_least_thm >> fs [] >>
-          irule least_pred_thm >> fs []
-      in
-        save_goal_and_prove (tm, prove_tac)
-      end
-  in
-    map prove_thm (zip pred_defs (zip fuel_def_tms (zip least_fuel_mono_thms
-                   (zip least_pred_thms (zip pred_n_imp_pred_least_thms raw_defs)))))
-  end
-
-(*
-val pred_imp_fuel_eq_raw_defs =
-  prove_pred_imp_fuel_eq_raw_defs
-    pred_defs fuel_def_tms least_fuel_mono_thms least_pred_thms
-    pred_n_imp_pred_least_thms raw_defs
- *)
-
-
-(* Generate "expand" definitions of the following shape (we use them to
-   hide the raw function bodies, to control the rewritings):
-
-   {[
-     even___expand even odd i : bool result =
-       if i = 0 then Return T else odd (i - 1)
-   ]}
-
-   {[
-     odd___expand even odd i : bool result =
-       if i = 0 then Return F else even (i - 1)
-   ]}
-
- *)
-fun gen_expand_defs (def_tms : term list) =
-  let
-    (* Generate the variables for “even”, “odd”, etc. *)
-    val fun_vars = map (fst o strip_comb o lhs) def_tms
-    val fun_tys = map type_of fun_vars
-    (* Generate the expansion *)
-    fun mk_def (def_tm : term) : thm =
-      let
-        val (exp_fun, args) = (strip_comb o lhs) def_tm
-        val (exp_fun_str, exp_fun_ty) = dest_var exp_fun
-        val exp_fun_str = exp_fun_str ^ expand_suffix
-        val exp_fun_ty = list_mk_arrow fun_tys exp_fun_ty
-        val exp_fun = mk_var (exp_fun_str, exp_fun_ty)
-        val exp_fun = list_mk_comb (exp_fun, fun_vars)
-        val exp_fun = list_mk_comb (exp_fun, args)
-        val tm = mk_eq (exp_fun, rhs def_tm)
-      in
-        Define ‘^tm’
-      end
-  in
-    map mk_def def_tms
-  end
-
-(*
-val def_tm = hd def_tms
-
-val expand_defs = gen_expand_defs def_tms
-*)
-
-(* Small utility:
-
-   Return the list:
-   {[
-     (“even___P i n”, “even i = even___expand even odd i”),
-     ...
-   ]}
-   
- *)
-fun mk_termination_diverge_tms
-  (def_tms : term list)
-  (pred_defs : thm list)
-  (raw_defs : thm list)
-  (expand_defs : thm list) :
-  (term * term) list =
-  let
-    (* Create the substitution for the "expand" functions:
-       {[
-         even -> even
-         odd -> odd
-         ...
-       ]}
-
-       where on the left we have *variables* and on the right we have
-       the "raw" definitions.
-     *)
-    fun mk_fun_subst (def_tm, raw_def) =
-      let
-        val var = (fst o strip_comb o lhs) def_tm
-        val f = (fst o strip_comb o lhs o snd o strip_forall o concl) raw_def
-      in
-        (var |-> f)
-      end
-    val fun_subst = map mk_fun_subst (zip def_tms raw_defs)
-  
-    fun mk_tm (pred_def, (raw_def, expand_def)) :
-      term * term =
-      let
-        (* “even___P i n” *)
-        val pred_tm = (lhs o snd o strip_forall o concl) pred_def
-        (* “even i = even___expand even odd i” *)
-        val expand_tm = (lhs o snd o strip_forall o concl) expand_def
-        val expand_tm = subst fun_subst expand_tm
-        val fun_tm = (lhs o snd o strip_forall o concl) raw_def
-        val fun_eq_tm = mk_eq (fun_tm, expand_tm)
-      in (pred_tm, fun_eq_tm) end
-  in
-    map mk_tm (zip pred_defs (zip raw_defs expand_defs))
-  end
-
-(*
-val term_div_tms =
-  mk_termination_diverge_tms pred_defs raw_defs expand_defs
-*)
-
-(* Prove the termination lemmas:
-   
-   {[
-     !i.
-       (?n. even___P i n) ==>
-         even i = even___expand even odd i
-   ]}
- *)
-fun prove_termination_thms
-  (term_div_tms : (term * term) list)
-  (fuel_defs : thm list)
-  (pred_defs : thm list)
-  (raw_defs : thm list)
-  (expand_defs : thm list)
-  (pred_n_imp_pred_least_thms : thm list)
-  (pred_imp_fuel_eq_raw_defs : thm list)
-  : thm list =
-  let
-    (* Create a map from functions in the recursive group to lemmas
-       to apply *)
-    fun mk_rec_fun_eq_pair (fuel_def, eq_th) =
-      let
-        val rfun = (get_fun_name_from_app o lhs o snd o strip_forall o concl) fuel_def
-      in
-        (rfun, eq_th)
-      end
-    val rec_fun_eq_map =
-      Redblackmap.fromList const_name_compare (
-        map mk_rec_fun_eq_pair
-          (zip fuel_defs pred_imp_fuel_eq_raw_defs))
-
-    (* Small tactic which rewrites the recursive calls *)
-    fun rewrite_rec_call (asms, g) =
-      let
-        val scrut = (strip_all_cases_get_scrutinee o lhs) g
-        val fun_id = get_fun_name_from_app scrut (* This can fail *)
-        (* This can raise an exception - hence the handle at the end
-           of the function *)
-        val eq_th = Redblackmap.find (rec_fun_eq_map, fun_id)
-        val eq_th = (UNDISCH_ALL o SPEC_ALL) eq_th
-        (* Match the theorem *)
-        val eq_th_tm = (lhs o concl) eq_th
-        val (var_s, ty_s) = match_term eq_th_tm scrut
-        val eq_th = INST var_s (INST_TYPE ty_s eq_th)
-        val eq_th = thm_to_conj_implies eq_th
-        (* Some tactics *)
-        val premise_tac = fs pred_defs >> fs [is_diverge_def]
-      in
-        (* Apply the theorem, prove the premise, and rewrite *)
-        (prove_premise_then premise_tac assume_tac eq_th >> fs []) (asms, g)
-      end handle NotFound => all_tac (asms, g)
-          | HOL_ERR _ => all_tac (asms, g) (* Getting the function name can also fail *)
-  
-    fun prove_one ((pred_tm, fun_eq_tm), pred_n_imp_pred_least_thm) :
-      thm =
-      let
-        (* “?n. even___P i n” *)
-        val pred_tm = mk_exists (fuel_var0, pred_tm)
-        (* “even i = even___expand even odd i” *)
-        val tm = fun_eq_tm
-        (* Add the implication *)
-        val tm = mk_imp (pred_tm, tm)
-        (* Quantify *)
-        val (_, args) = strip_comb (lhs fun_eq_tm)
-        val tm = list_mk_forall (args, tm)
-
-        (* Prove *)
-        val prove_tac =
-          rpt gen_tac >>
-          disch_tac >>
-
-          (* Expand the raw definition and get rid of the ‘?n ...’ *)
-          pure_once_rewrite_tac raw_defs >>
-          pure_asm_rewrite_tac [] >>
-
-          (* Simplify *)
-          fs [] >>
-
-          (* Prove that: “even___P i $(LEAST ...)” *)
-          imp_res_tac pred_n_imp_pred_least_thm >>
-
-          (* We don't need the ‘even___P i n’ assumption anymore: we have a more
-             precise one with the least upper bound *)
-          last_x_assum ignore_tac >>
-
-          (* Expand *)
-          fs pred_defs >>
-          fs [is_diverge_def] >>
-          fs expand_defs >>
-
-          (* We need to be a bit careful when expanding the definitions which use fuel:
-             it can make the simplifier loop. *)
-          rpt (pop_assum mp_tac) >>
-          pure_once_rewrite_tac fuel_defs >>
-          rpt disch_tac >>
-
-          (* Expand the binds *)
-          fs [bind_def, case_result_same_eq] >>
-
-          (* Explore all the paths by doing case disjunctions *)
-          rpt (rewrite_rec_call >> case_progress >> fs [case_result_same_eq])
-      in
-        save_goal_and_prove (tm, prove_tac)
-      end
-  in
-    map prove_one
-      (zip term_div_tms pred_n_imp_pred_least_thms)
-  end
-
-(*
-val termination_thms =
-  prove_termination_thms term_div_tms fuel_defs pred_defs
-    raw_defs expand_defs pred_n_imp_pred_least_thms
-    pred_imp_fuel_eq_raw_defs
-
-val ((pred_tm, fun_eq_tm), pred_n_imp_pred_least_thm) = hd (zip term_div_tms pred_n_imp_pred_least_thms)
-set_goal ([], tm)
-*)
-
-(* Prove the divergence lemmas:
-
-   {[
-     !i.
-       (!n. ~even___P i n) ==>
-        (!n. ~even___P i (SUC n)) ==>
-         even i = even___expand even odd i
-   ]}
-
-   Note that the shape of the theorem is very precise: this helps for the proof.
-   Also, by correctly ordering the assumptions, we make sure that by rewriting
-   we don't convert one of the two to “T”.
- *)
-fun prove_divergence_thms
-  (term_div_tms : (term * term) list)
-  (fuel_defs : thm list)
-  (pred_defs : thm list)
-  (raw_defs : thm list)
-  (expand_defs : thm list)
-  : thm list =
-  let
-    (* Create a set containing the names of all the functions in the recursive group *)
-    fun get_rec_fun_id (fuel_def : thm) =
-     (get_fun_name_from_app o lhs o snd o strip_forall o concl) fuel_def
-    val rec_fun_set =
-      Redblackset.fromList const_name_compare (
-        map get_rec_fun_id raw_defs)
-
-    (* Small tactic which rewrites the recursive calls *)
-    fun rewrite_rec_call (asms, g) =
-      let
-        val scrut = (strip_all_cases_get_scrutinee o lhs) g
-        val fun_id = get_fun_name_from_app scrut (* This can fail *)
-      in
-        (* Check if the function is part of the group we are considering *)
-        if Redblackset.member (rec_fun_set, fun_id) then
-          let
-            (* Create a subgoal “odd i = Diverge” *)
-            val ret_ty = (hd o snd o dest_type o type_of) scrut
-            val g = mk_eq (scrut, mk_diverge_tm ret_ty)
-
-            (* Create a subgoal: “?n. odd___P i n”.
-
-               It is a bit cumbersome because we have to lookup the proper
-               predicate (from “odd” we need to lookup “odd___P”) and we
-               may have to perform substitutions... We hack a bit by using
-               a conversion to rewrite “odd i” to a term which contains
-               the “?n. odd___P i n” we are looking for.
-             *)
-            val exists_g = (rhs o concl) (PURE_REWRITE_CONV raw_defs scrut)
-            val (_, exists_g, _) = TypeBase.dest_case exists_g
-            (* The tactic to prove the subgoal *)
-            val prove_sg_tac =
-              pure_rewrite_tac raw_defs >>
-              Cases_on ‘^exists_g’ >> pure_asm_rewrite_tac [] >> fs [] >>
-              (* There must only remain the positive case (i.e., “?n. ...”):
-                 we have a contradiction *)
-              exfalso >>
-              (* The end of the proof is done by opening the definitions *)
-              pop_assum mp_tac >>
-              fs pred_defs >> fs [is_diverge_def]
-          in
-            (SUBGOAL_THEN g assume_tac >- prove_sg_tac >> fs []) (asms, g)
-          end
-        else all_tac (asms, g) (* Nothing to do *)
-      end handle HOL_ERR _ => all_tac (asms, g)
-  
-    fun prove_one (pred_tm, fun_eq_tm) :
-      thm =
-      let
-        (* “!n. ~even___P i n” *)
-        val neg_pred_tm = mk_neg pred_tm
-        val pred_tm = mk_forall (fuel_var0, neg_pred_tm)
-        val pred_suc_tm = subst [fuel_var0 |-> numSyntax.mk_suc fuel_var0] neg_pred_tm
-        val pred_suc_tm = mk_forall (fuel_var0, pred_suc_tm)
-
-        (* “even i = even___expand even odd i” *)
-        val tm = fun_eq_tm
-
-        (* Add the implications *)
-        val tm = list_mk_imp ([pred_tm, pred_suc_tm], tm)
-
-        (* Quantify *)
-        val (_, args) = strip_comb (lhs fun_eq_tm)
-        val tm = list_mk_forall (args, tm)
-
-        (* Prove *)
-        val prove_tac =
-          rpt gen_tac >>
-
-          pure_rewrite_tac raw_defs >>
-          rpt disch_tac >>
-
-          (* This allows to simplify the “?n. even___P i n” *)
-          fs [] >>
-          (* We don't need the last assumption anymore *)
-          last_x_assum ignore_tac >>
-
-          (* Expand *)
-          fs pred_defs >> fs [is_diverge_def] >>
-          fs expand_defs >>
-
-          (* We need to be a bit careful when expanding the definitions which use fuel:
-             it can make the simplifier loop.
-           *)
-          pop_assum mp_tac >>
-          pure_once_rewrite_tac fuel_defs  >>
-          rpt disch_tac >> fs [bind_def, case_result_same_eq] >>
-
-          (* Evaluate all the paths *)
-          rpt (rewrite_rec_call >> case_progress >> fs [case_result_same_eq])
-      in
-        save_goal_and_prove (tm, prove_tac)
-      end
-  in
-    map prove_one term_div_tms
-  end
-
-(*
-val (pred_tm, fun_eq_tm) = hd term_div_tms
-set_goal ([], tm)
-
-val divergence_thms =
-  prove_divergence_thms
-    term_div_tms
-    fuel_defs
-    pred_defs
-    raw_defs
-    expand_defs
-*)
-
-(* Prove the final lemmas:
-
-   {[
-     !i. even i = even___expand even odd i
-   ]}
-
-   Note that the shape of the theorem is very precise: this helps for the proof.
-   Also, by correctly ordering the assumptions, we make sure that by rewriting
-   we don't convert one of the two to “T”.
- *)
-fun prove_final_eqs
-  (term_div_tms : (term * term) list)
-  (termination_thms : thm list)
-  (divergence_thms : thm list)
-  (raw_defs : thm list)
-  : thm list =
-  let
-    fun prove_one ((pred_tm, fun_eq_tm), (termination_thm, divergence_thm)) : thm =
-      let
-        val (_, args) = strip_comb (lhs fun_eq_tm)
-        val g = list_mk_forall (args, fun_eq_tm)
-        (* We make a case disjunction of the subgoal: “exists n. even___P i n” *)
-        val exists_g = (rhs o concl) (PURE_REWRITE_CONV raw_defs (lhs fun_eq_tm))
-        val (_, exists_g, _) = TypeBase.dest_case exists_g
-        val prove_tac =
-          rpt gen_tac >>
-          Cases_on ‘^exists_g’
-          >-( (* Termination *)
-             irule termination_thm >> pure_asm_rewrite_tac [])
-          (* Divergence *)
-          >> irule divergence_thm >> fs []
-          
-      in
-        save_goal_and_prove (g, prove_tac)
-      end    
-  in
-    map prove_one (zip term_div_tms (zip termination_thms divergence_thms))
-  end
-
-(*
-val termination_thm = hd termination_thms
-val divergence_thm = hd divergence_thms
-set_goal ([], g)
-*)
-
-(* The final function: define potentially diverging functions in an error monad *)
 fun DefineDiv (def_qt : term quotation) =
   let
-    (* Parse the definitions.
-    
-       Example:
-       {[
-         (even (i : int) : bool result = if i = 0 then Return T else odd (i - 1)) /\
-         (odd (i : int) : bool result = if i = 0 then Return F else even (i - 1))
-       ]}
-     *)
+    (* Parse the definitions *)
     val def_tms = (strip_conj o list_mk_conj o rev) (Defn.parse_quote def_qt)
 
-    (* Generate definitions which use some fuel
+    (* Compute the names and the input/output types of the functions *)
+    fun compute_names_in_out_tys (tm : term) : string * (hol_type * hol_type) =
+      let
+        val app = lhs tm
+        val name = (fst o dest_var o fst o strip_comb) app
+        val out_ty = dest_result (type_of app)
+        val input_tys = pairSyntax.list_mk_prod (map type_of ((snd o strip_comb) app))
+      in
+        (name, (input_tys, out_ty))
+      end
+    val (fnames, in_out_tys) = unzip (map compute_names_in_out_tys def_tms)
+
+    (* Generate the body to give to the fixed-point operator *)
+    val body = mk_body fnames in_out_tys def_tms
+
+    (* Prove that the body satisfies the validity property required by the fixed point *)
+    val body_is_valid = prove_body_is_valid body
     
-       Example:
-       {[
-         even___fuel n i =
-           case fuel of
-             0 => Diverge
-           | SUC fuel => 
-             if i = 0 then Return T else odd_fuel (i - 1))
-       ]}
-     *)
-     val fuel_defs = mk_fuel_defs def_tms
+    (* Generate the definitions for the various functions by using the fixed point
+       and the body *)
+    val raw_defs = mk_raw_defs in_out_tys def_tms body_is_valid
 
-     (* Generate the predicate definitions.
-     
-        {[ even___P n i = = ~is_diverge (even___fuel n i) ]}
-      *)
-     val fuel_def_tms = map (snd o strip_forall o concl) fuel_defs
-     val pred_defs = map mk_fuel_predicate_defs (zip def_tms fuel_def_tms)
-     
-     (* Prove the monotonicity property for the fuel, all at once
-
-      *)
-     val fuel_mono_thm = prove_fuel_mono pred_defs fuel_defs
-     
-     (* Prove the individual fuel functions - TODO: update
-
-        {[
-          !n i. $LEAST (even___P i) <= n ==> even___fuel n i = even___fuel ($LEAST (even___P i)) i
-        ]}
-      *)
-     val least_fuel_mono_thms = prove_least_fuel_mono pred_defs fuel_mono_thm
-
-     (*
-       {[
-         !n i. even___P i n ==> $LEAST (even___P i) <= n
-       ]}
-      *)
-     val least_pred_thms = prove_least_pred_thms pred_defs
-
-     (*
-       {[
-         !n i. even___P i n ==> even___P i ($LEAST (even___P i))
-       ]}
-      *)
-     val pred_n_imp_pred_least_thms = prove_pred_n_imp_pred_least_thms pred_defs
-
-     (*
-       "Raw" definitions:
-
-       {[
-         even i = if (?n. even___P i n) then even___P ($LEAST (even___P i)) i else Diverge
-       ]}
-      *)
-     val raw_defs = define_raw_defs def_tms pred_defs fuel_defs
-
-     (*
-       !n i. even___P i n ==> even___fuel n i = even i
-      *)
-     val pred_imp_fuel_eq_raw_defs =
-       prove_pred_imp_fuel_eq_raw_defs
-         pred_defs fuel_def_tms least_fuel_mono_thms
-         least_pred_thms pred_n_imp_pred_least_thms raw_defs
-
-     (* "Expand" definitions *)
-     val expand_defs = gen_expand_defs def_tms
-
-     (* Small utility *)
-     val term_div_tms = mk_termination_diverge_tms def_tms pred_defs raw_defs expand_defs
-
-     (* Termination theorems *)
-     val termination_thms =
-       prove_termination_thms term_div_tms fuel_defs pred_defs
-         raw_defs expand_defs pred_n_imp_pred_least_thms pred_imp_fuel_eq_raw_defs
-
-     (* Divergence theorems *)
-     val divergence_thms =
-       prove_divergence_thms term_div_tms fuel_defs pred_defs raw_defs expand_defs
-
-     (* Final theorems:
-
-        {[
-          ∀i. even i = even___E even odd i,
-          ⊢ ∀i. odd i = odd___E even odd i
-        ]}
-      *)
-     val final_eqs = prove_final_eqs term_div_tms termination_thms divergence_thms raw_defs
-     val final_eqs = map (PURE_REWRITE_RULE expand_defs) final_eqs
+    (* Prove the final equations *)
+    val def_eqs = prove_def_eqs body_is_valid def_tms raw_defs
   in
-    (* We return the final equations, which act as rewriting theorems *)
-    final_eqs
+    def_eqs
   end
 
 end
